reconstruct RelocProgSemantics

assembler/RelocProgGlobalenvs.v
@@ -76,3 +76,2598 @@ End GENV.
 End Genv.
 
 Coercion Genv.genv_senv: Genv.t >-> Senv.t.
+
+(** Global environments for RelocProg which parameterizes the data type *)
+
+Section INSTRSIZE.
+
+Variable instr_size : instruction -> Z.
+
+(**Initialization of the global environment *)
+Definition gen_global (id:ident) (e:symbentry) : (block*ptrofs) :=
+  match e.(symbentry_secindex) with
+  | secindex_normal sec =>
+    (Global sec, Ptrofs.repr e.(symbentry_value))
+  | _ =>
+    (Global id, Ptrofs.zero)
+  end.
+
+Definition gen_symb_map (symbtbl: symbtable) : PTree.t (block * ptrofs) :=
+  PTree.map gen_global symbtbl.
+
+
+Definition acc_instr_map r (i:instruction) :=
+  let '(ofs, map) := r in
+  let map' := fun o => if Ptrofs.eq_dec ofs o then Some i else (map o) in
+  let ofs' := Ptrofs.add ofs (Ptrofs.repr (instr_size i)) in
+  (ofs', map').
+
+Definition gen_instr_map (c:code) :=
+  let '(_, map) := fold_left acc_instr_map c (Ptrofs.zero, fun o => None) in
+  map.
+
+Definition acc_code_map {D: Type} r (id:ident) (sec:RelocProg.section instruction D) :=
+  match sec with
+  | sec_text c =>
+    NMap.set _ (Global id) (gen_instr_map c) r
+  | _ => r
+  end.
+
+Definition gen_code_map {D: Type} (sectbl: RelocProg.sectable instruction D) :=
+  PTree.fold acc_code_map sectbl (NMap.init _ (fun o => None)).
+
+Definition acc_extfuns (idg: ident * gdef) extfuns :=
+  let '(id, gdef) := idg in
+  match gdef with
+  | Gfun (External ef) => NMap.set  _ (Global id) (Some ef) extfuns
+  | _ => extfuns
+  end.
+
+Definition gen_extfuns (idgs: list (ident * gdef)) :=
+  fold_right acc_extfuns (NMap.init _ None) idgs.
+
+Lemma PTree_Properteis_of_list_get_extfuns : forall defs i f,
+    list_norepet (map fst defs) ->
+    (PTree_Properties.of_list defs) ! i = (Some (Gfun (External f))) ->
+    (gen_extfuns defs) (Global i) = Some f.
+Proof.
+  induction defs as [|def defs].
+  - cbn. intros. rewrite PTree.gempty in H0. congruence.
+  - intros i f NORPT OF. destruct def as (id, def).
+    inv NORPT.
+    destruct (ident_eq id i).
+    + subst. erewrite PTree_Properties_of_list_cons in OF; auto.
+      inv OF. cbn. rewrite NMap.gss. auto.
+    + erewrite PTree_Properties_of_list_tail in OF; eauto.
+      cbn. repeat (destr; eauto; subst).
+      erewrite NMap.gso;auto.
+      unfold not. intros. inv H;congruence.
+Qed.
+
+Definition globalenv {D: Type} (p: RelocProg.program fundef unit instruction D) : Genv.t :=
+  let symbmap := gen_symb_map (prog_symbtable p) in
+  let imap := gen_code_map (prog_sectable p) in
+  let extfuns := gen_extfuns p.(prog_defs) in
+  Genv.mkgenv symbmap extfuns imap p.(prog_senv).
+
+
+(* properteis of instruction map *)
+Lemma gen_instr_map_inv_aux: forall n c ofs i ofs1 m1,
+    length c = n ->
+    fold_left acc_instr_map c
+              (Ptrofs.zero, fun _ : ptrofs => None) = (ofs1,m1) ->
+    m1 ofs = Some i ->
+    In i c.
+Proof.
+  induction n;intros.
+  rewrite length_zero_iff_nil in H. subst.
+  simpl in H0. inv H0.  inv H1.
+  
+  exploit LocalLib.length_S_inv;eauto.
+  intros (l' & a1 & A1 & B1). subst.
+  clear H.
+  rewrite fold_left_app in H0. simpl in H0.
+  destruct ((fold_left acc_instr_map l'
+            (Ptrofs.zero, fun _ : ptrofs => None))) eqn: FOLD.
+  unfold acc_instr_map in H0 at 1. inv H0.
+  destr_in H1.
+  + inv H1. apply in_app.
+    right. constructor. auto.
+  +  apply in_app. left. eapply IHn;eauto.
+Qed.
+
+Lemma gen_instr_map_inv: forall c ofs i,
+    gen_instr_map c ofs = Some i ->
+    In i c.
+Proof.
+  unfold gen_instr_map. intros.
+  destruct (fold_left acc_instr_map c (Ptrofs.zero, fun _ : ptrofs => None)) eqn: FOLD.
+  eapply gen_instr_map_inv_aux;eauto.
+Qed.
+
+
+(* code map = code *)
+Lemma gen_code_map_inv: forall D (sectbl : RelocProg.sectable instruction D) b ofs i,
+    (gen_code_map sectbl) b ofs = Some i ->
+    (exists id c, b = Global id /\ sectbl ! id = Some (sec_text c) /\ In i c).
+Proof.
+  unfold gen_code_map. intros.
+  rewrite PTree.fold_spec in H.
+  assert (exists id c, b = Global id /\ In (id, sec_text c) (PTree.elements sectbl) /\ In i c).
+  { set (l:= (PTree.elements sectbl)) in *.
+    generalize H.
+    generalize l i ofs b.
+    clear H l i ofs b. clear sectbl.
+    intro l.
+    assert (LEN: exists n, length l = n).
+    { induction l. exists O. auto.
+      destruct IHl.
+      eexists. simpl. auto. }
+
+    destruct LEN. generalize x l H.
+    clear H x l.
+    induction x;intros.
+    rewrite length_zero_iff_nil in H. subst.
+    simpl in H0. rewrite NMap.gi in H0. inv H0.
+
+    exploit LocalLib.length_S_inv;eauto.
+    intros (l' & a1 & A1 & B1). subst.
+    clear H.
+    rewrite fold_left_app in H0.
+    simpl in H0. destruct a1. simpl in *.
+    destruct (eq_block (Global p) b);subst.
+    - destruct s;simpl in H0.
+      + rewrite NMap.gss in H0.
+        exists p, code. split;eauto.
+        rewrite in_app_iff. split. right. constructor.
+        auto. eapply gen_instr_map_inv. eauto.
+      + eapply IHx in H0;eauto.
+        destruct H0 as (id & c & P1 & P2 & P3).
+        inv P1. exists id,c.
+        split;auto. split;auto.
+        apply in_app.
+        left. auto.
+      + eapply IHx in H0;eauto.
+        destruct H0 as (id & c & P1 & P2 & P3).
+        inv P1. exists id,c.
+        split;auto. split;auto.
+        apply in_app.
+        left. auto.
+    - destruct s;simpl in H0.
+      + rewrite NMap.gso in H0;auto.
+        eapply IHx in H0;eauto.
+        destruct H0 as (id & c & P1 & P2 & P3).
+        inv P1. exists id,c.
+        split;auto. split;auto.
+        apply in_app.
+        left. auto.
+      + eapply IHx in H0;eauto.
+        destruct H0 as (id & c & P1 & P2 & P3).
+        inv P1. exists id,c.
+        split;auto. split;auto.
+        apply in_app.
+        left. auto.
+      + eapply IHx in H0;eauto.
+        destruct H0 as (id & c & P1 & P2 & P3).
+        inv P1. exists id,c.
+        split;auto. split;auto.
+        apply in_app.
+        left. auto.   }
+  destruct H0 as (id & c & P1 & P2 & P3).
+  exists id,c. split;auto. split;auto.
+  apply PTree.elements_complete.
+  auto.
+Qed.
+
+
+(** Initialization of memory *)
+Section WITHGE1.
+
+Variable ge:Genv.t.
+
+(* Since we use a new global environment, we need to redefine the storing of the init data *)
+Definition store_init_data (m: mem) (b: block) (p: Z) (id: init_data) : option mem :=
+  match id with
+  | Init_int8 n => Mem.store Mint8unsigned m b p (Vint n)
+  | Init_int16 n => Mem.store Mint16unsigned m b p (Vint n)
+  | Init_int32 n => Mem.store Mint32 m b p (Vint n)
+  | Init_int64 n => Mem.store Mint64 m b p (Vlong n)
+  | Init_float32 n => Mem.store Mfloat32 m b p (Vsingle n)
+  | Init_float64 n => Mem.store Mfloat64 m b p (Vfloat n)
+  | Init_addrof gloc ofs =>
+    (* match Genv.find_symbol ge gloc with *)
+    (* | None => None *)
+    (* | Some (b',ofs') => Mem.store Mptr m b p (Vptr b' (Ptrofs.add ofs ofs')) *)
+    (* end       *)
+    Mem.store Mptr m b p (Genv.symbol_address ge gloc ofs)
+  (* store zero to common data, which simplify the relocbingenproof, but make symbtablegenproof harder *)
+  | Init_space n => store_zeros m b p (Z.max n 0)
+  end.
+
+Fixpoint store_init_data_list (m: mem) (b: block) (p: Z) (idl: list init_data)
+                              {struct idl}: option mem :=
+  match idl with
+  | nil => Some m
+  | id :: idl' =>
+      match store_init_data m b p id with
+      | None => None
+      | Some m' => store_init_data_list m' b (p + init_data_size id) idl'
+      end
+  end.
+
+(* Allocation of external and common symbols *)
+Definition alloc_external_comm_symbol (r: option mem) (id: ident) (e:symbentry): option mem :=
+  match r with
+  | None => None
+  | Some m =>
+  match symbentry_type e with
+  | symb_notype => None
+  (* impossible *)
+  (* match symbentry_secindex e with *)
+    (* | secindex_undef => *)
+    (*   let (m1, b) := Mem.alloc_glob id m 0 0 in Some m1 *)
+    (* | _ => None *)
+    (* end *)
+  | symb_func =>
+    match symbentry_secindex e with
+    | secindex_undef =>
+      let (m1, b) := Mem.alloc_glob id m 0 1 in
+      Mem.drop_perm m1 b 0 1 Nonempty
+    | secindex_comm =>
+      None (**r Impossible *)
+    | secindex_normal _ => Some m
+    end
+  | symb_data =>
+    match symbentry_secindex e with
+    | secindex_undef =>
+      (* let sz := symbentry_size e in *)
+      let (m1, b) := Mem.alloc_glob id m 0 1 in
+      match store_zeros m1 b 0 1 with
+      | None => None
+      | Some m2 =>
+        Mem.drop_perm m2 b 0 1 Nonempty
+      end
+    | secindex_comm =>
+      let sz := Z.max (symbentry_size e) 0 in
+      let (m1, b) := Mem.alloc_glob id m 0 sz in
+      match store_zeros m1 b 0 sz with
+      | None => None
+      | Some m2 =>
+       (* writable for common symbol *)
+        Mem.drop_perm m2 b 0 sz Writable
+      end        
+    | secindex_normal _ => Some m
+    end
+  end
+end.
+
+Definition alloc_external_symbols (m: mem) (t: symbtable) : option mem :=
+  PTree.fold alloc_external_comm_symbol t (Some m).
+
+(* Allocation of sections *)
+Definition alloc_section (r: option mem) (id: ident) (sec: section) : option mem :=
+  match r with
+  | None => None
+  | Some m =>
+    let sz := sec_size instr_size sec in
+    match sec with
+      | sec_rwdata init =>
+        let '(m1, b) := Mem.alloc_glob id m 0 sz in
+        match store_zeros m1 b 0 sz with
+        | None => None
+        | Some m2 =>
+          match store_init_data_list m2 b 0 init with
+          | None => None
+          | Some m3 => Mem.drop_perm m3 b 0 sz Writable
+          end       
+        end
+      | sec_rodata init =>
+        let '(m1, b) := Mem.alloc_glob id m 0 sz in
+        match store_zeros m1 b 0 sz with
+        | None => None
+        | Some m2 =>
+          match store_init_data_list m2 b 0 init with
+          | None => None
+          | Some m3 => Mem.drop_perm m3 b 0 sz Readable
+          end
+        end
+      | sec_text code =>        
+        let (m1, b) := Mem.alloc_glob id m 0 (Z.max sz 1) in
+        Mem.drop_perm m1 b 0 (Z.max sz 1 )Nonempty
+    end
+  end.
+
+Definition alloc_sections (sectbl: sectable) (m:mem) :option mem :=
+  PTree.fold alloc_section sectbl (Some m).
+
+(** init data to bytes *)
+Definition bytes_of_init_data (i: init_data): list memval :=
+  match i with
+  | Init_int8 n => inj_bytes (encode_int 1%nat (Int.unsigned n))
+  | Init_int16 n => inj_bytes (encode_int 2%nat (Int.unsigned n))
+  | Init_int32 n => inj_bytes (encode_int 4%nat (Int.unsigned n))
+  | Init_int64 n => inj_bytes (encode_int 8%nat (Int64.unsigned n))
+  | Init_float32 n => inj_bytes (encode_int 4%nat (Int.unsigned (Float32.to_bits n)))
+  | Init_float64 n => inj_bytes (encode_int 8%nat (Int64.unsigned (Float.to_bits n)))
+  | Init_space n => list_repeat (Z.to_nat n) (Byte Byte.zero)
+  | Init_addrof id ofs =>
+      match Genv.find_symbol ge id with
+      | Some (b,ofs') => inj_value (if Archi.ptr64 then Q64 else Q32) (Vptr b (Ptrofs.add ofs ofs'))
+      | None   => list_repeat (if Archi.ptr64 then 8%nat else 4%nat) Undef
+      end
+  end.
+
+Fixpoint bytes_of_init_data_list (il: list init_data): list memval :=
+  match il with
+  | nil => nil
+  | i :: il => bytes_of_init_data i ++ bytes_of_init_data_list il
+  end.
+
+(** load_store_init_data *)
+Fixpoint load_store_init_data (m: mem) (b: block) (p: Z) (il: list init_data) {struct il} : Prop :=
+  match il with
+  | nil => True
+  | Init_int8 n :: il' =>
+      Mem.load Mint8unsigned m b p = Some(Vint(Int.zero_ext 8 n))
+      /\ load_store_init_data m b (p + 1) il'
+  | Init_int16 n :: il' =>
+      Mem.load Mint16unsigned m b p = Some(Vint(Int.zero_ext 16 n))
+      /\ load_store_init_data m b (p + 2) il'
+  | Init_int32 n :: il' =>
+      Mem.load Mint32 m b p = Some(Vint n)
+      /\ load_store_init_data m b (p + 4) il'
+  | Init_int64 n :: il' =>
+      Mem.load Mint64 m b p = Some(Vlong n)
+      /\ load_store_init_data m b (p + 8) il'
+  | Init_float32 n :: il' =>
+      Mem.load Mfloat32 m b p = Some(Vsingle n)
+      /\ load_store_init_data m b (p + 4) il'
+  | Init_float64 n :: il' =>
+      Mem.load Mfloat64 m b p = Some(Vfloat n)
+      /\ load_store_init_data m b (p + 8) il'
+  | Init_addrof symb ofs :: il' =>
+      ((exists b' ofs', Genv.find_symbol ge symb = Some (b',ofs') /\ Mem.load Mptr m b p = Some(Vptr b' (Ptrofs.add ofs ofs'))) \/ (Genv.find_symbol ge symb = None /\ Mem.load Mptr m b p = Some Vundef))
+      /\ load_store_init_data m b (p + size_chunk Mptr) il'
+  | Init_space n :: il' =>
+      Globalenvs.Genv.read_as_zero m b p (Z.max n 0)
+      /\ load_store_init_data m b (p + Z.max n 0) il'
+  end.
+
+
+
+(* unchanged properties *)
+
+Remark store_init_data_unchanged:
+  forall (P: block -> Z -> Prop) b i m p m',
+  store_init_data m b p i = Some m' ->
+  (forall ofs, p <= ofs < p + init_data_size i -> ~ P b ofs) ->
+  Mem.unchanged_on P m m'.
+Proof.
+  intros. destruct i;simpl in *.
+  1-7 :try (eapply Mem.store_unchanged_on; eauto; fail).  
+  eapply Genv.store_zeros_unchanged;eauto.
+  (* Mptr: auto would simplify ptr.64 and I don't know how to solve it (Opaque dose not work) *)
+  eapply Mem.store_unchanged_on. eauto.
+  unfold Mptr. destruct Archi.ptr64;simpl;auto.
+Qed.
+
+Remark store_init_data_list_unchanged:
+  forall (P: block -> Z -> Prop) b il m p m',
+  store_init_data_list m b p il = Some m' ->
+  (forall ofs, p <= ofs -> ~ P b ofs) ->
+  Mem.unchanged_on P m m'.
+Proof.
+  induction il; simpl; intros.
+- inv H. apply Mem.unchanged_on_refl.
+- destruct (store_init_data m b p a) as [m1|] eqn:?; try congruence.
+  apply Mem.unchanged_on_trans with m1.
+  eapply store_init_data_unchanged; eauto. intros; apply H0; tauto.
+  eapply IHil; eauto. intros; apply H0. generalize (init_data_size_pos a); lia.
+Qed.
+
+
+
+Lemma store_init_data_loadbytes:
+  forall m b p i m',
+  store_init_data m b p i = Some m' ->
+  Mem.loadbytes m' b p (init_data_size i) = Some (bytes_of_init_data i).
+Proof.
+  intros; destruct i; simpl in H; try apply (Mem.loadbytes_store_same _ _ _ _ _ _ H).
+  -  simpl.
+     assert (EQ: Z.of_nat (Z.to_nat z) = Z.max z 0).
+     { destruct (zle 0 z). rewrite Z2Nat.id; extlia. destruct z; try discriminate. simpl. extlia. }
+     rewrite <- EQ.
+     eapply Genv.store_zeros_loadbytes in H.
+     apply H. lia. simpl. lia.
+- rewrite Genv.init_data_size_addrof. simpl.
+  unfold Genv.symbol_address in H.
+  destruct (Genv.find_symbol ge i) as [b'|]; try discriminate.
+  destruct b'.
+  rewrite (Mem.loadbytes_store_same _ _ _ _ _ _ H).
+  unfold encode_val, Mptr; destruct Archi.ptr64; reflexivity.
+  
+  rewrite (Mem.loadbytes_store_same _ _ _ _ _ _ H).
+  unfold encode_val,Mptr. destruct Archi.ptr64;auto.
+Qed.
+
+Lemma store_init_data_list_loadbytes:
+  forall b il m p m',
+  store_init_data_list m b p il = Some m' ->
+  Mem.loadbytes m' b p (init_data_list_size il) = Some (bytes_of_init_data_list il).
+Proof.
+  induction il as [ | i1 il]; simpl; intros.
+- apply Mem.loadbytes_empty. lia.
+- generalize (init_data_size_pos i1) (init_data_list_size_pos il); intros P1 PL.
+  destruct (store_init_data m b p i1) as [m1|] eqn:S; try discriminate.
+  apply Mem.loadbytes_concat.
+  eapply Mem.loadbytes_unchanged_on with (P := fun b1 ofs1 => ofs1 < p + init_data_size i1).
+  eapply store_init_data_list_unchanged; eauto.
+  intros; lia.
+  intros; lia.
+  eapply store_init_data_loadbytes; eauto.
+  (* red; intros; apply H0. lia. lia. *)
+  apply IHil with m1; auto.
+  lia. lia.
+  (* red; intros. *)
+  (* eapply Mem.loadbytes_unchanged_on with (P := fun b1 ofs1 => p + init_data_size i1 <= ofs1). *)
+  (* eapply store_init_data_unchanged; eauto. *)
+  (* intros; lia. *)
+  (* intros; lia. *)
+  (* apply H0. lia. lia. *)
+  (* auto. auto. *)
+Qed.
+
+
+Lemma store_init_data_list_charact:
+  forall b il m p m',
+  store_init_data_list m b p il = Some m' ->
+  (* Genv.read_as_zero m b p (init_data_list_size il) -> *)
+  load_store_init_data m' b p il.
+Proof.
+  assert (A: forall chunk v m b p m1 il m',
+    Mem.store chunk m b p v = Some m1 ->
+    store_init_data_list m1 b (p + size_chunk chunk) il = Some m' ->
+    Mem.load chunk m' b p = Some(Val.load_result chunk v)).
+  {
+    intros.
+    eapply Mem.load_unchanged_on with (P := fun b' ofs' => ofs' < p + size_chunk chunk).
+    eapply store_init_data_list_unchanged; eauto. intros; lia.
+    intros; tauto.
+    eapply Mem.load_store_same; eauto.
+  }  induction il; simpl.
+- auto.
+- intros. destruct (store_init_data m b p a) as [m1|] eqn:?; try congruence.
+  exploit IHil; eauto.
+  (* set (P := fun (b': block) ofs' => p + init_data_size a <= ofs'). *)
+  (* apply Genv.read_as_zero_unchanged with (m := m) (P := P). *)
+  (* (* red; *) intros; (* apply H0; *) auto. (* generalize (init_data_size_pos a); lia. lia. *) *)
+  (* eapply store_init_data_unchanged with (P := P); eauto. *)
+  (* intros; unfold P. lia. *)
+  (* intros; unfold P. lia. *)
+  (* intro D. *)
+  intros.
+  destruct a; simpl in Heqo.
++ split; auto. eapply (A Mint8unsigned (Vint i)); eauto.
++ split; auto. eapply (A Mint16unsigned (Vint i)); eauto.
++ split; auto. eapply (A Mint32 (Vint i)); eauto.
++ split; auto. eapply (A Mint64 (Vlong i)); eauto.
++ split; auto. eapply (A Mfloat32 (Vsingle f)); eauto.
++ split; auto. eapply (A Mfloat64 (Vfloat f)); eauto.
++ split; auto.
+  set (P := fun (b': block) ofs' => ofs' < p + init_data_size (Init_space z)).
+  (* inv Heqo. *) apply Genv.read_as_zero_unchanged with (m := m1) (P := P).
+  eapply Genv.store_zeros_read_as_zero;eauto.
+  
+  (* red; intros. apply H0; auto. simpl. generalize (init_data_list_size_pos il); extlia. *)
+  eapply store_init_data_list_unchanged; eauto.
+  intros; unfold P. lia.
+  intros; unfold P. simpl; extlia.
++ rewrite Genv.init_data_size_addrof in *.
+  split; auto.
+
+  unfold Genv.symbol_address in *.
+  
+  destruct (Genv.find_symbol ge i); try congruence.
+  destruct p0.
+  
+  left. exists b0,i1; split; auto.
+  transitivity (Some (Val.load_result Mptr (Vptr b0 (Ptrofs.add i0 i1)))).
+  eapply (A Mptr (Vptr b0 (Ptrofs.add i0 i1))); eauto.
+  unfold Val.load_result, Mptr; destruct Archi.ptr64; auto.
+  
+  right. split;auto.
+  transitivity (Some (Val.load_result Mptr Vundef)).
+  eapply (A Mptr Vundef); eauto.
+  unfold Val.load_result, Mptr; destruct Archi.ptr64; auto.
+Qed.
+
+
+Remark load_store_init_data_invariant:
+  forall m m' b,
+  (forall chunk ofs, Mem.load chunk m' b ofs = Mem.load chunk m b ofs) ->
+  forall il p,
+  load_store_init_data m b p il -> load_store_init_data m' b p il.
+Proof.
+  induction il; intro p; simpl.
+  auto.
+  rewrite ! H. destruct a; intuition. red; intros; rewrite H; auto.
+Qed.
+
+
+End WITHGE1.
+
+Section INITDATA.
+
+Variable ge: Genv.t.
+
+Remark store_init_data_perm:
+  forall k prm b' q i b m p m',
+  store_init_data ge m b p i = Some m' ->
+  (Mem.perm m b' q k prm <-> Mem.perm m' b' q k prm).
+Proof.
+  intros. 
+  assert (forall chunk v,
+          Mem.store chunk m b p v = Some m' ->
+          (Mem.perm m b' q k prm <-> Mem.perm m' b' q k prm)).
+    intros; split; eauto with mem.
+    destruct i; simpl in H; eauto.
+  eapply Genv.store_zeros_perm.
+  eauto.
+
+  (* destruct (Genv.find_symbol ge i); try discriminate. destruct p0. eauto. *)
+Qed.
+
+Remark store_init_data_list_perm:
+  forall k prm b' q idl b m p m',
+  store_init_data_list ge m b p idl = Some m' ->
+  (Mem.perm m b' q k prm <-> Mem.perm m' b' q k prm).
+Proof.
+  induction idl as [ | i1 idl]; simpl; intros.
+- inv H; tauto.
+- destruct (store_init_data ge m b p i1) as [m1|] eqn:S1; try discriminate.
+  transitivity (Mem.perm m1 b' q k prm). 
+  eapply store_init_data_perm; eauto.
+  eapply IHidl; eauto.
+Qed.
+
+Lemma store_init_data_exists:
+  forall m b p i,
+    Mem.range_perm m b p (p + init_data_size i) Cur Writable ->
+    (* Mem.stack_access (Mem.stack m) b p (p + init_data_size i)  -> *)
+    (Genv.init_data_alignment i | p) ->
+    (* (forall id ofs, i = Init_addrof id ofs -> exists b ofs', Genv.find_symbol ge id = Some (b,ofs')) -> *)
+    exists m', store_init_data ge m b p i = Some m'.
+Proof.
+  intros. 
+  assert (DFL: forall chunk v,
+          init_data_size i = size_chunk chunk ->
+          Genv.init_data_alignment i = align_chunk chunk ->
+          exists m', Mem.store chunk m b p v = Some m').
+  { intros. destruct (Mem.valid_access_store m chunk b p v) as (m' & STORE).
+    split. rewrite <- H1; auto.
+    rewrite  <- H2. auto.
+    exists m'; auto. }
+  destruct i.
+  1-7: eauto.
+  (* store zero *)
+  simpl. eapply Genv.store_zeros_exists.
+  simpl in H. auto.
+
+  (* Mptr *)
+  simpl. eapply DFL.
+  unfold Mptr. simpl. destruct Archi.ptr64;auto.
+  unfold Mptr. simpl. destruct Archi.ptr64;auto.
+  (* simpl. exploit H1; eauto. intros (b1 & OFS & FS). rewrite FS. eapply DFL. *)
+  (* unfold init_data_size, Mptr. destruct Archi.ptr64; auto. *)
+  (* unfold Genv.init_data_alignment, Mptr. destruct Archi.ptr64; auto. *)                                                            
+Qed.
+
+(* SACC
+Lemma store_init_data_stack_access:
+  forall m b p i1 m1,
+    store_init_data ge m b p i1 = Some m1 ->
+    forall b' lo hi,
+      stack_access (Mem.stack m1) b' lo hi <-> stack_access (Mem.stack m) b' lo hi.
+Proof.
+  unfold store_init_data.
+  destruct i1; intros; try now (eapply Mem.store_stack_access ; eauto).
+  inv H; tauto.
+Qed.
+*)
+
+Lemma store_init_data_list_exists:
+  forall b il m p,
+  Mem.range_perm m b p (p + init_data_list_size il) Cur Writable ->
+  (* stack_access (Mem.stack m) b p (p + init_data_list_size il) -> *)
+  Genv.init_data_list_aligned p il ->
+  (* (forall id ofs, In (Init_addrof id ofs) il -> exists b ofs', Genv.find_symbol ge id = Some (b,ofs')) -> *)
+  exists m', store_init_data_list ge m b p il = Some m'.
+Proof.
+  induction il as [ | i1 il ]; simpl; intros.
+- exists m; auto.
+- destruct H0. 
+  destruct (@store_init_data_exists m b p i1) as (m1 & S1); eauto.
+  red; intros. apply H. generalize (init_data_list_size_pos il); lia.
+  (* generalize (init_data_list_size_pos il); omega. *)
+  rewrite S1.
+  apply IHil; eauto.
+  red; intros. erewrite <- store_init_data_perm by eauto. apply H. generalize (init_data_size_pos i1); lia.
+Qed.
+
+Remark store_init_data_load_other:
+  forall b' i b m p m' chunk ofs,
+  store_init_data ge m b p i = Some m' -> b <> b' ->
+  (Mem.load chunk m b' ofs = Mem.load chunk m' b' ofs).
+Proof.
+  intros.
+  assert (forall chunk' v,
+          Mem.store chunk' m b p v = Some m' -> b <> b' ->
+          (Mem.load chunk m b' ofs = Mem.load chunk m' b' ofs)).
+   { intros. eapply Mem.load_store_other in H1; eauto. }
+   destruct i. 1-7:  simpl in H; eauto.
+   2: simpl in H; eauto.
+
+   eapply Genv.store_zeros_load_other;eauto.
+   
+  (* destruct (Genv.find_symbol ge i); try discriminate. destruct p0. eauto. *)
+Qed.
+
+Remark store_init_data_list_load_other:
+  forall b' idl b m p m' chunk ofs,
+  store_init_data_list ge m b p idl = Some m' -> b <> b' ->
+  (Mem.load chunk m b' ofs = Mem.load chunk m' b' ofs).
+Proof.
+  induction idl as [ | i1 idl]; simpl; intros.
+- inv H; tauto.
+- destruct (store_init_data ge m b p i1) as [m1|] eqn:S1; try discriminate.
+  transitivity (Mem.load chunk m1 b' ofs).
+  eapply store_init_data_load_other; eauto.
+  eapply IHidl; eauto.
+Qed.
+
+Remark store_init_data_loadbytes_other:
+  forall b' i b m p m' lo hi,
+  store_init_data ge m b p i = Some m' -> b <> b' ->
+  (Mem.loadbytes m b' lo hi = Mem.loadbytes m' b' lo hi).
+Proof.
+  intros.
+  assert (forall chunk' v,
+          Mem.store chunk' m b p v = Some m' -> b <> b' ->
+          (Mem.loadbytes m b' lo hi = Mem.loadbytes m' b' lo hi)).
+  { intros. eapply Mem.loadbytes_store_other in H1; eauto. }
+  destruct i. 1-7:  simpl in H; eauto.
+   2: simpl in H; eauto
+.
+   eapply Genv.store_zeros_loadbytes_other;eauto.
+   (* destruct (Genv.find_symbol ge i); try discriminate. destruct p0. eauto.    *)
+Qed.
+
+Remark store_init_data_list_loadbytes_other:
+  forall b' idl b m p m' lo hi,
+  store_init_data_list ge m b p idl = Some m' -> b <> b' ->
+  (Mem.loadbytes m b' lo hi= Mem.loadbytes m' b' lo hi).
+Proof.
+  induction idl as [ | i1 idl]; simpl; intros.
+- inv H; tauto.
+- destruct (store_init_data ge m b p i1) as [m1|] eqn:S1; try discriminate.
+  transitivity (Mem.loadbytes m1 b' lo hi).
+  eapply store_init_data_loadbytes_other; eauto.
+  eapply IHidl; eauto.
+Qed.
+
+End INITDATA.
+
+
+(** globals_initialized, which is similar to the 'globals_initialized' in Globalenv.v. It is used to establish the relation between the programs and their initialized memory  *)
+Definition globals_initialized (ge: Genv.t) (prog: program) (m:mem):=
+  forall id b ofs0,
+    (* b = Global id -> *)
+    Genv.find_symbol ge id = Some (b,ofs0) ->
+    let ofs0 := Ptrofs.unsigned ofs0 in
+    match prog.(prog_sectable) ! id with
+    | Some sec =>
+      (* ofs0 = 0 /\ : required if supporting section merging *)
+      match sec with
+      | sec_text code =>
+        Mem.perm m b ofs0 Cur Nonempty /\
+        let sz := Z.max (code_size instr_size code) 1 in
+        (forall ofs k p, Mem.perm m b (ofs0+ofs) k p -> 0 <= ofs < sz /\ p = Nonempty)
+      | sec_rodata data =>        
+        let sz := (init_data_list_size data) in
+        Mem.range_perm m b ofs0 sz Cur Readable /\ (forall ofs k p, Mem.perm m b (ofs0+ofs) k p -> 0 <= ofs < sz /\ perm_order Readable p)
+        /\ load_store_init_data ge m b ofs0 data
+        /\ Mem.loadbytes m b ofs0 sz = Some (bytes_of_init_data_list ge data)
+      | sec_rwdata data =>
+        let sz := (init_data_list_size data) in
+        Mem.range_perm m b ofs0 sz Cur Writable /\ (forall ofs k p, Mem.perm m b (ofs0+ofs) k p -> 0 <= ofs < sz /\ perm_order Writable p)
+        /\ load_store_init_data ge m b ofs0 data
+        /\ Mem.loadbytes m b ofs0 sz = Some (bytes_of_init_data_list ge data)
+      end
+    | None =>
+      (* common symbol or external function *)
+      match prog.(prog_symbtable) ! id with
+      | Some e =>
+        match e.(symbentry_type),e.(symbentry_secindex) with
+        | symb_func,secindex_undef =>
+          Mem.perm m b 0 Cur Nonempty /\
+          (forall ofs k p, Mem.perm m b ofs k p -> ofs = 0 /\ p = Nonempty)
+        | symb_data,secindex_comm =>
+          let sz := e.(symbentry_size) in
+          let data := Init_space sz :: nil in
+          let sz' := Z.max sz 0 in
+          Mem.range_perm m b 0 sz' Cur Writable /\ (forall ofs k p, Mem.perm m b ofs k p -> 0 <= ofs < sz' /\ perm_order Writable p)
+          /\ load_store_init_data ge m b 0 data
+          /\ Mem.loadbytes m b 0 sz' = Some (bytes_of_init_data_list ge data)
+        | symb_data,secindex_undef =>
+          Mem.perm m b 0 Cur Nonempty /\
+          (forall ofs k p, Mem.perm m b ofs k p -> ofs = 0 /\ p = Nonempty)
+        (* when id resides in a location of a section *)
+        (* if id <> i then in secidx is allowed: the following cases are required *)
+        | _,_ => False
+        end
+      | _ => False
+      end
+    end.
+
+
+(* The memory initialization: first allocate the sections and then allocate the external and common symbols *)
+Definition init_mem (p: program) :=
+  let ge := globalenv p in
+  match alloc_sections ge p.(prog_sectable) Mem.empty with
+  | Some m1 =>
+    alloc_external_symbols m1 p.(prog_symbtable)
+  | None => None
+  end.
+
+
+(** Start to prove the initialization of memory confirms to the global_initialized: lemma called init_mem_characterization_gen  *)
+
+Definition well_formed_symbtbl (sectbl:sectable) symbtbl:=
+  forall id e,
+    symbtbl ! id = Some e ->
+    match symbentry_secindex e with
+    | secindex_normal i =>        
+      symbentry_type e <> symb_notype
+      /\ i = id                  (* does not support sections merging *)
+      /\ (exists sec, sectbl ! i = Some sec
+                /\ sec_size instr_size sec = symbentry_size e
+                /\ symbentry_value e = 0)
+                (* separation: it should be more complicate. If include the restriction list below, the globals_initialized should be enhanced *)
+                (* (i <> id -> (0 <= symbentry_value e + symbentry_size e <= sec_size instr_size sec))) *)
+    | secindex_comm =>
+      symbentry_type e = symb_data /\ sectbl ! id = None
+    | secindex_undef =>
+      symbentry_type e <> symb_notype /\ sectbl ! id = None
+    end.
+
+Definition globals_initialized_sections ge m b sec :=
+  match sec with
+  | sec_text code =>
+    Mem.perm m b 0 Cur Nonempty /\
+    (let sz := Z.max (code_size instr_size code) 1 in
+     forall (ofs : Z) (k : perm_kind) (p : permission), Mem.perm m b ofs k p -> 0 <= ofs < sz /\ p = Nonempty)
+  | sec_rwdata data =>
+    let sz := init_data_list_size data in
+    Mem.range_perm m b 0 sz Cur Writable /\
+    (forall (ofs : Z) (k : perm_kind) (p : permission),
+        Mem.perm m b ofs k p -> 0 <= ofs < sz /\ perm_order Writable p) /\
+    load_store_init_data ge m b 0 data /\ Mem.loadbytes m b 0 sz = Some (bytes_of_init_data_list ge data)
+  | sec_rodata data =>
+    let sz := init_data_list_size data in
+    Mem.range_perm m b 0 sz Cur Readable /\
+    (forall (ofs : Z) (k : perm_kind) (p : permission),
+        Mem.perm m b ofs k p -> 0 <= ofs < sz /\ perm_order Readable p) /\
+    load_store_init_data ge m b 0 data /\ Mem.loadbytes m b 0 sz = Some (bytes_of_init_data_list ge data)
+  end.                                                                       
+
+Definition globals_initialized_external ge m b e:=
+  match e.(symbentry_type),e.(symbentry_secindex) with
+  | symb_func,secindex_undef =>
+    Mem.perm m b 0 Cur Nonempty /\
+    (forall ofs k p, Mem.perm m b ofs k p -> ofs = 0 /\ p = Nonempty)
+  | symb_data,secindex_comm =>
+    let sz := e.(symbentry_size) in
+    let data := Init_space sz :: nil in
+    let sz' := Z.max sz 0 in
+    Mem.range_perm m b 0 sz' Cur Writable /\ (forall ofs k p, Mem.perm m b ofs k p -> 0 <= ofs < sz' /\ perm_order Writable p)
+    /\ load_store_init_data ge m b 0 data
+    /\ Mem.loadbytes m b 0 sz' = Some (bytes_of_init_data_list ge data)
+  | symb_data,secindex_undef =>
+    Mem.perm m b 0 Cur Nonempty /\
+    (forall ofs k p, Mem.perm m b ofs k p -> ofs = 0 /\ p = Nonempty)
+  | _,_ => False
+  end.
+
+(* alloc_glob dose not change the globals_initialized_sections *)
+Lemma alloc_glob_pres_globals_initialized_sections: forall b b' id lo hi sec m1 m2 ge,
+    globals_initialized_sections ge m1 b sec ->
+    Mem.alloc_glob id m1 lo hi = (m2,b') ->
+    b <> b' ->
+    globals_initialized_sections ge m2 b sec.
+Proof.
+  unfold globals_initialized_sections.
+  intros.
+  exploit Mem.alloc_glob_result;eauto;intros. subst.  
+  destruct sec.
+  - destruct H. split. 
+    + eapply Mem.perm_alloc_glob_1 in H0. eapply H0.
+      eauto.
+      congruence.
+    + intros.
+      assert (Mem.perm m1 b ofs k p).
+      eapply Mem.perm_alloc_glob_1 in H0. eapply H0.
+      auto.
+      congruence. eapply H2 in H4.
+      eauto.
+  - destruct H as (P1 & P2 & P3 & P4).
+    split.
+    (* 1 *)
+    unfold Mem.range_perm. intros.
+    eapply Mem.perm_alloc_glob_1 in H0. eapply H0.
+    eauto.
+    congruence.
+    (* 2 *)
+    split.
+    intros.
+    assert (Mem.perm m1 b ofs k p).
+    eapply Mem.perm_alloc_glob_1 in H0. eapply H0.                   
+    auto.
+    congruence. eapply P2 in H2.
+    eauto.
+    (* 3 *)
+    split.
+    eapply load_store_init_data_invariant.
+    2: eapply P3. intros.
+    eapply Mem.load_alloc_glob_unchanged;eauto.
+    (* 4 *)   
+    erewrite Mem.loadbytes_alloc_glob_unchanged;eauto.
+    
+  - destruct H as (P1 & P2 & P3 & P4).
+    split.
+    (* 1 *)
+    unfold Mem.range_perm. intros.
+    eapply Mem.perm_alloc_glob_1 in H0. eapply H0.
+    eauto.
+    congruence.
+    (* 2 *)
+    split.
+    intros.
+    assert (Mem.perm m1 b ofs k p).
+    eapply Mem.perm_alloc_glob_1 in H0. eapply H0.                   
+    auto.
+    congruence. eapply P2 in H2.
+    eauto.
+    (* 3 *)
+    split.
+    eapply load_store_init_data_invariant.
+    2: eapply P3. intros.
+    eapply Mem.load_alloc_glob_unchanged;eauto.
+    (* 4 *)   
+    erewrite Mem.loadbytes_alloc_glob_unchanged;eauto.
+Qed.
+
+
+Lemma alloc_glob_pres_globals_initialized_external: forall b b' id lo hi e m1 m2 ge,
+    globals_initialized_external ge m1 b e ->
+    Mem.alloc_glob id m1 lo hi = (m2,b') ->
+    b <> b' ->
+    globals_initialized_external ge m2 b e.
+Proof.
+  unfold globals_initialized_external.
+  intros.
+  exploit Mem.alloc_glob_result;eauto;intros. subst.  
+  destr.
+  - destr.
+    destruct H. split.
+    + eapply Mem.perm_alloc_glob_1 in H0. eapply H0.
+      eauto.
+      congruence.
+    + intros.
+      assert (Mem.perm m1 b ofs k p).
+      eapply Mem.perm_alloc_glob_1 in H0. eapply H0.
+      auto.
+      congruence. eapply H2 in H4.
+      eauto.
+  - destr.
+    + destruct H as (P1 & P2 & P3 & P4).
+      split.
+      (* 1 *)
+      unfold Mem.range_perm. intros.
+      eapply Mem.perm_alloc_glob_1 in H0. eapply H0.
+      eauto.
+      congruence.
+      (* 2 *)
+      split.
+      intros.
+      assert (Mem.perm m1 b ofs k p).
+      eapply Mem.perm_alloc_glob_1 in H0. eapply H0.                   
+      auto.
+      congruence. eapply P2 in H2.
+      eauto.
+      (* 3 *)
+      split.
+      eapply load_store_init_data_invariant.
+      2: eapply P3. intros.
+      eapply Mem.load_alloc_glob_unchanged;eauto.
+      (* 4 *)   
+      erewrite Mem.loadbytes_alloc_glob_unchanged;eauto.
+    + destruct H. split.
+      * eapply Mem.perm_alloc_glob_1 in H0. eapply H0.
+        eauto.
+        congruence.
+      * intros.
+        assert (Mem.perm m1 b ofs k p).
+        eapply Mem.perm_alloc_glob_1 in H0. eapply H0.
+        auto.
+        congruence. eapply H2 in H4.
+        eauto.
+Qed.
+
+
+Lemma store_zeros_pres_globals_initialized_sections: forall b b' sz ofs sec m1 m2 ge,
+    globals_initialized_sections ge m1 b sec ->
+    store_zeros m1 b' ofs sz = Some m2 ->
+    b <> b' ->
+    globals_initialized_sections ge m2 b sec.
+Proof.
+  unfold globals_initialized_sections.
+  intros.
+  destruct sec.
+  - destruct H.
+    split.
+    + erewrite <- Genv.store_zeros_perm;eauto.
+    + intros.
+      assert (Mem.perm m1 b ofs0 k p).
+      eapply Genv.store_zeros_perm;eauto.
+      eapply H2 in H4.
+      eauto.
+  - destruct H as (P1 & P2 & P3 & P4).
+    split.
+    (* 1 *)
+    unfold Mem.range_perm in *.
+    intros.
+    erewrite <- Genv.store_zeros_perm;eauto. 
+    (* 2 *)
+    split.
+    intros.
+    assert (Mem.perm m1 b ofs0 k p).
+    eapply Genv.store_zeros_perm;eauto.
+    eapply P2 in H2.
+    eauto.
+    (* 3 *)
+    split.
+    eapply load_store_init_data_invariant.
+    2: eapply P3.
+    intros.
+    erewrite <- (Genv.store_zeros_load_other m1);eauto.
+    (* 4 *)        
+    erewrite <- Genv.store_zeros_loadbytes_other;eauto.
+
+  - destruct H as (P1 & P2 & P3 & P4).
+    split.
+    (* 1 *)
+    unfold Mem.range_perm in *.
+    intros.
+    erewrite <- Genv.store_zeros_perm;eauto. 
+    (* 2 *)
+    split.
+    intros.
+    assert (Mem.perm m1 b ofs0 k p).
+    eapply Genv.store_zeros_perm;eauto.
+    eapply P2 in H2.
+    eauto.
+    (* 3 *)
+    split.
+    eapply load_store_init_data_invariant.
+    2: eapply P3.
+    intros.
+    erewrite <- (Genv.store_zeros_load_other m1);eauto.
+    (* 4 *)        
+    erewrite <- Genv.store_zeros_loadbytes_other;eauto.
+Qed.
+
+
+Lemma store_zeros_pres_globals_initialized_external: forall b b' sz ofs e m1 m2 ge,
+    globals_initialized_external ge m1 b e ->
+    store_zeros m1 b' ofs sz = Some m2 ->
+    b <> b' ->
+    globals_initialized_external ge m2 b e.
+Proof.
+  unfold globals_initialized_external.
+  intros.
+  destr.
+  - destr. destruct H. split.
+    + erewrite <- Genv.store_zeros_perm;eauto.
+    + intros.
+      assert (Mem.perm m1 b ofs0 k p).
+      eapply Genv.store_zeros_perm;eauto.
+      eapply H2 in H4.
+      eauto.
+  - destr. destruct H as (P1 & P2 & P3 & P4).
+    split.
+    (* 1 *)
+    unfold Mem.range_perm in *.
+    intros.
+    erewrite <- Genv.store_zeros_perm;eauto. 
+    (* 2 *)
+    split.
+    intros.
+    assert (Mem.perm m1 b ofs0 k p).
+    eapply Genv.store_zeros_perm;eauto.
+    eapply P2 in H2.
+    eauto.
+    (* 3 *)
+    split.
+    eapply load_store_init_data_invariant.
+    2: eapply P3.
+    intros.
+    erewrite <- (Genv.store_zeros_load_other m1);eauto.
+    (* 4 *)        
+    erewrite <- Genv.store_zeros_loadbytes_other;eauto.
+
+     destruct H. split.
+    + erewrite <- Genv.store_zeros_perm;eauto.
+    + intros.
+      assert (Mem.perm m1 b ofs0 k p).
+      eapply Genv.store_zeros_perm;eauto.
+      eapply H2 in H4.
+      eauto.
+Qed.
+
+
+Lemma drop_pres_globals_initialized_sections: forall b b' lo hi p sec m1 m2 ge,
+    globals_initialized_sections ge m1 b sec ->
+    Mem.drop_perm m1 b' lo hi p = Some m2 ->
+    b <> b' ->
+    globals_initialized_sections ge m2 b sec.
+Proof.
+  unfold globals_initialized_sections.
+  intros.
+  destruct sec.
+  - destruct H. split.
+    + eapply Mem.perm_drop_3;eauto.
+    + intros.
+      assert (Mem.perm m1 b ofs k p0).
+      eapply Mem.perm_drop_4;eauto.
+      eapply H2 in H4.
+      eauto.
+  - destruct H as (P1 & P2 & P3 & P4).
+    split.
+    (* 1 *)
+    unfold Mem.range_perm in *.
+    intros.
+    eapply Mem.perm_drop_3;eauto.
+    (* 2 *)
+    split.
+    intros.
+    assert (Mem.perm m1 b ofs k p0).
+    eapply Mem.perm_drop_4;eauto.
+    eapply P2 in H2.
+    eauto.
+    (* 3 *)
+    split.
+    eapply load_store_init_data_invariant.
+    2: eapply P3. intros.
+    erewrite (Mem.load_drop m1);eauto.
+    (* 4 *)
+    erewrite Mem.loadbytes_drop;eauto.
+
+- destruct H as (P1 & P2 & P3 & P4).
+    split.
+    (* 1 *)
+    unfold Mem.range_perm in *.
+    intros.
+    eapply Mem.perm_drop_3;eauto.
+    (* 2 *)
+    split.
+    intros.
+    assert (Mem.perm m1 b ofs k p0).
+    eapply Mem.perm_drop_4;eauto.
+    eapply P2 in H2.
+    eauto.
+    (* 3 *)
+    split.
+    eapply load_store_init_data_invariant.
+    2: eapply P3. intros.
+    erewrite (Mem.load_drop m1);eauto.
+    (* 4 *)
+    erewrite Mem.loadbytes_drop;eauto.
+Qed.
+
+
+Lemma drop_pres_globals_initialized_external: forall b b' lo hi p e m1 m2 ge,
+    globals_initialized_external ge m1 b e ->
+    Mem.drop_perm m1 b' lo hi p = Some m2 ->
+    b <> b' ->
+    globals_initialized_external ge m2 b e.
+Proof.
+  unfold globals_initialized_external.
+  intros.
+  destr.
+  - destr. destruct H. split.
+    + eapply Mem.perm_drop_3;eauto.
+    + intros.
+      assert (Mem.perm m1 b ofs k p0).
+      eapply Mem.perm_drop_4;eauto.
+      eapply H2 in H4.
+      eauto.
+  - destr.
+    destruct H as (P1 & P2 & P3 & P4).
+    split.
+    (* 1 *)
+    unfold Mem.range_perm in *.
+    intros.
+    eapply Mem.perm_drop_3;eauto.
+    (* 2 *)
+    split.
+    intros.
+    assert (Mem.perm m1 b ofs k p0).
+    eapply Mem.perm_drop_4;eauto.
+    eapply P2 in H2.
+    eauto.
+    (* 3 *)
+    split.
+    eapply load_store_init_data_invariant.
+    2: eapply P3. intros.
+    erewrite (Mem.load_drop m1);eauto.
+    (* 4 *)
+    erewrite Mem.loadbytes_drop;eauto.
+    
+    destruct H. split.
+    + eapply Mem.perm_drop_3;eauto.
+    + intros.
+      assert (Mem.perm m1 b ofs k p0).
+      eapply Mem.perm_drop_4;eauto.
+      eapply H2 in H4.
+      eauto.
+Qed.      
+
+     
+    
+(* FIXME: so verbose and we should use the above lemma to simplify it *)
+Lemma alloc_sections_none: forall secs ge,
+    fold_left
+      (fun (a : option mem) (p0 : positive * section) => alloc_section ge a (fst p0) (snd p0))
+      secs None = None.
+Proof.
+  induction secs;simpl;auto.
+Qed.
+
+Lemma alloc_sections_pres_characterization: forall secs sec ge m0 m id ,
+    ~ In id  (map fst secs) ->
+    globals_initialized_sections ge m0 (Global id) sec ->
+    fold_left
+      (fun (a : option mem) (p0 : positive * section) => alloc_section ge a (fst p0) (snd p0))
+      secs (Some m0) = Some m ->
+    globals_initialized_sections ge m (Global id) sec.
+Proof.
+  induction secs;simpl;intros.
+  inv H1. auto.
+  eapply Decidable.not_or in H.
+  destruct H.
+  destruct a. simpl in *.
+  destruct s;simpl in *.
+  - destruct (Mem.alloc_glob i m0 0 (Z.max (code_size instr_size code) 1)) eqn:ALLOC.
+    destruct ((Mem.drop_perm m1 b 0 (Z.max (code_size instr_size code) 1) Nonempty)) eqn:DROP.
+    assert (globals_initialized_sections ge m2 (Global id) sec).
+    { unfold globals_initialized_sections.
+      unfold globals_initialized_sections in H0.
+      destruct sec.
+      - destruct H0. split.
+        + eapply Mem.perm_drop_3;eauto.
+          left. eapply Mem.alloc_glob_result in ALLOC.
+          subst. congruence.
+          eapply Mem.perm_alloc_glob_1 in ALLOC. eapply ALLOC.
+          eauto.
+          congruence.
+        + intros.
+          assert (Mem.perm m0 (Global id) ofs k p).
+          eapply Mem.perm_alloc_glob_1 in ALLOC. eapply ALLOC.                   
+          eapply Mem.perm_drop_4;eauto.
+          congruence. eapply H3 in H5.
+          eauto.
+      - destruct H0 as (P1 & P2 & P3 & P4).
+        split.
+        (* 1 *)
+        unfold Mem.range_perm in *.
+        intros.
+        eapply Mem.perm_drop_3;eauto.
+        left. eapply Mem.alloc_glob_result in ALLOC.
+        subst. congruence.
+        eapply Mem.perm_alloc_glob_1 in ALLOC. eapply ALLOC.
+        eauto.
+        congruence.
+        (* 2 *)
+        split.
+        intros.
+        assert (Mem.perm m0 (Global id) ofs k p).
+        eapply Mem.perm_alloc_glob_1 in ALLOC. eapply ALLOC.                   
+        eapply Mem.perm_drop_4;eauto.
+        congruence. eapply P2 in H3.
+        eauto.
+        (* 3 *)
+        split.
+        eapply load_store_init_data_invariant.
+        2: eapply P3. intros.
+        erewrite (Mem.load_drop m1);eauto.
+        erewrite Mem.load_alloc_glob_unchanged;eauto.
+        congruence. left.
+        eapply Mem.alloc_glob_result in ALLOC.
+        subst. congruence.
+        (* 4 *)
+        erewrite Mem.loadbytes_drop. 2: eapply DROP.        
+        erewrite Mem.loadbytes_alloc_glob_unchanged;eauto.
+        congruence. left.
+        eapply Mem.alloc_glob_result in ALLOC.
+        subst. congruence.
+      - destruct H0 as (P1 & P2 & P3 & P4).
+        split.
+        (* 1 *)
+        unfold Mem.range_perm in *.
+        intros.
+        eapply Mem.perm_drop_3;eauto.
+        left. eapply Mem.alloc_glob_result in ALLOC.
+        subst. congruence.
+        eapply Mem.perm_alloc_glob_1 in ALLOC. eapply ALLOC.
+        eauto.
+        congruence.
+        (* 2 *)
+        split.
+        intros.
+        assert (Mem.perm m0 (Global id) ofs k p).
+        eapply Mem.perm_alloc_glob_1 in ALLOC. eapply ALLOC.                   
+        eapply Mem.perm_drop_4;eauto.
+        congruence. eapply P2 in H3.
+        eauto.
+        (* 3 *)
+        split.
+        eapply load_store_init_data_invariant.
+        2: eapply P3. intros.
+        erewrite (Mem.load_drop m1);eauto.
+        erewrite Mem.load_alloc_glob_unchanged;eauto.
+        congruence. left.
+        eapply Mem.alloc_glob_result in ALLOC.
+        subst. congruence.
+        (* 4 *)
+        erewrite Mem.loadbytes_drop. 2: eapply DROP.        
+        erewrite Mem.loadbytes_alloc_glob_unchanged;eauto.
+        congruence. left.
+        eapply Mem.alloc_glob_result in ALLOC.
+        subst. congruence. }
+    eapply IHsecs;eauto.
+    rewrite alloc_sections_none in H1. congruence.
+
+  - destruct (Mem.alloc_glob i m0 0 (init_data_list_size init)) eqn:ALLOC.
+    destr_in H1.
+    2: { rewrite alloc_sections_none in H1. congruence. }
+    destr_in H1.
+    2: { rewrite alloc_sections_none in H1. congruence. }
+    destruct (Mem.drop_perm m3 b 0 (init_data_list_size init) Writable) eqn:DROP.
+    2: { rewrite alloc_sections_none in H1. congruence. }    
+    assert (globals_initialized_sections ge m4 (Global id) sec).
+    { unfold globals_initialized_sections.
+      unfold globals_initialized_sections in H0.
+      destruct sec.
+      - destruct H0. split.
+        + eapply Mem.perm_drop_3;eauto.
+          left. eapply Mem.alloc_glob_result in ALLOC.
+          subst. congruence.
+          erewrite <- store_init_data_list_perm. 2: eapply Heqo0.
+          erewrite <- Genv.store_zeros_perm. 2: eapply Heqo.          
+          eapply Mem.perm_alloc_glob_1 in ALLOC. eapply ALLOC.
+          eauto.
+          congruence.
+        + intros.
+          assert (Mem.perm m0 (Global id) ofs k p).
+          eapply Mem.perm_alloc_glob_1 in ALLOC. eapply ALLOC.
+          eapply Genv.store_zeros_perm;eauto.
+          eapply store_init_data_list_perm;eauto.
+          eapply Mem.perm_drop_4;eauto.
+          congruence. eapply H3 in H5.
+          eauto.
+      - destruct H0 as (P1 & P2 & P3 & P4).
+        split.
+        (* 1 *)
+        unfold Mem.range_perm in *.
+        intros.
+        eapply Mem.perm_drop_3;eauto.
+        left. eapply Mem.alloc_glob_result in ALLOC.
+        subst. congruence.
+        erewrite <- store_init_data_list_perm. 2: eapply Heqo0.
+        erewrite <- Genv.store_zeros_perm. 2: eapply Heqo.          
+        eapply Mem.perm_alloc_glob_1 in ALLOC. eapply ALLOC.
+        eauto.
+        congruence.
+        (* 2 *)
+        split.
+        intros.
+        assert (Mem.perm m0 (Global id) ofs k p).
+        eapply Mem.perm_alloc_glob_1 in ALLOC. eapply ALLOC.
+        eapply Genv.store_zeros_perm;eauto.
+        eapply store_init_data_list_perm;eauto.
+        eapply Mem.perm_drop_4;eauto.
+        congruence. eapply P2 in H3.
+        eauto.
+        (* 3 *)
+        split.
+        eapply load_store_init_data_invariant.
+        2: eapply P3. intros.
+        erewrite (Mem.load_drop m3);eauto.
+        erewrite <- store_init_data_list_load_other.
+        2: eapply Heqo0.
+        erewrite <- (Genv.store_zeros_load_other m1);eauto.
+        erewrite Mem.load_alloc_glob_unchanged;eauto.
+        congruence.
+        eapply Mem.alloc_glob_result in ALLOC. subst.
+        congruence.
+        eapply Mem.alloc_glob_result in ALLOC. subst.
+        congruence. 
+        left.
+        eapply Mem.alloc_glob_result in ALLOC.
+        subst. congruence.
+        (* 4 *)
+        erewrite Mem.loadbytes_drop. 2: eapply DROP.
+        erewrite <- store_init_data_list_loadbytes_other.
+        2: eapply Heqo0.
+        erewrite <- Genv.store_zeros_loadbytes_other.
+        2: eapply Heqo.        
+        erewrite Mem.loadbytes_alloc_glob_unchanged.
+        2: eapply ALLOC.
+        congruence. congruence. 
+        eapply Mem.alloc_glob_result in ALLOC.
+        subst. congruence.
+        eapply Mem.alloc_glob_result in ALLOC.
+        subst. congruence.
+        left.
+        eapply Mem.alloc_glob_result in ALLOC.
+        subst. congruence.
+      - destruct H0 as (P1 & P2 & P3 & P4).
+        split.
+        (* 1 *)
+        unfold Mem.range_perm in *.
+        intros.
+        eapply Mem.perm_drop_3;eauto.
+        left. eapply Mem.alloc_glob_result in ALLOC.
+        subst. congruence.
+        erewrite <- store_init_data_list_perm. 2: eapply Heqo0.
+        erewrite <- Genv.store_zeros_perm. 2: eapply Heqo.          
+        eapply Mem.perm_alloc_glob_1 in ALLOC. eapply ALLOC.
+        eauto.
+        congruence.
+        (* 2 *)
+        split.
+        intros.
+        assert (Mem.perm m0 (Global id) ofs k p).
+        eapply Mem.perm_alloc_glob_1 in ALLOC. eapply ALLOC.
+        eapply Genv.store_zeros_perm;eauto.
+        eapply store_init_data_list_perm;eauto.
+        eapply Mem.perm_drop_4;eauto.
+        congruence. eapply P2 in H3.
+        eauto.
+        (* 3 *)
+        split.
+        eapply load_store_init_data_invariant.
+        2: eapply P3. intros.
+        erewrite (Mem.load_drop m3);eauto.
+        erewrite <- store_init_data_list_load_other.
+        2: eapply Heqo0.
+        erewrite <- (Genv.store_zeros_load_other m1);eauto.
+        erewrite Mem.load_alloc_glob_unchanged;eauto.
+        congruence.
+        eapply Mem.alloc_glob_result in ALLOC. subst.
+        congruence.
+        eapply Mem.alloc_glob_result in ALLOC. subst.
+        congruence. 
+        left.
+        eapply Mem.alloc_glob_result in ALLOC.
+        subst. congruence.
+        (* 4 *)
+        erewrite Mem.loadbytes_drop. 2: eapply DROP.
+        erewrite <- store_init_data_list_loadbytes_other.
+        2: eapply Heqo0.
+        erewrite <- Genv.store_zeros_loadbytes_other.
+        2: eapply Heqo.        
+        erewrite Mem.loadbytes_alloc_glob_unchanged.
+        2: eapply ALLOC.
+        congruence. congruence. 
+        eapply Mem.alloc_glob_result in ALLOC.
+        subst. congruence.
+        eapply Mem.alloc_glob_result in ALLOC.
+        subst. congruence.
+        left.
+        eapply Mem.alloc_glob_result in ALLOC.
+        subst. congruence. }
+    eapply IHsecs;eauto.
+
+  - destruct (Mem.alloc_glob i m0 0 (init_data_list_size init)) eqn:ALLOC.
+    destr_in H1.
+    2: { rewrite alloc_sections_none in H1. congruence. }
+    destr_in H1.
+    2: { rewrite alloc_sections_none in H1. congruence. }
+    destruct (Mem.drop_perm m3 b 0 (init_data_list_size init) Readable) eqn:DROP.
+    2: { rewrite alloc_sections_none in H1. congruence. }    
+    assert (globals_initialized_sections ge m4 (Global id) sec).
+    { unfold globals_initialized_sections.
+      unfold globals_initialized_sections in H0.
+      destruct sec.
+      - destruct H0. split.
+        + eapply Mem.perm_drop_3;eauto.
+          left. eapply Mem.alloc_glob_result in ALLOC.
+          subst. congruence.
+          erewrite <- store_init_data_list_perm. 2: eapply Heqo0.
+          erewrite <- Genv.store_zeros_perm. 2: eapply Heqo.          
+          eapply Mem.perm_alloc_glob_1 in ALLOC. eapply ALLOC.
+          eauto.
+          congruence.
+        + intros.
+          assert (Mem.perm m0 (Global id) ofs k p).
+          eapply Mem.perm_alloc_glob_1 in ALLOC. eapply ALLOC.
+          eapply Genv.store_zeros_perm;eauto.
+          eapply store_init_data_list_perm;eauto.
+          eapply Mem.perm_drop_4;eauto.
+          congruence. eapply H3 in H5.
+          eauto.
+      - destruct H0 as (P1 & P2 & P3 & P4).
+        split.
+        (* 1 *)
+        unfold Mem.range_perm in *.
+        intros.
+        eapply Mem.perm_drop_3;eauto.
+        left. eapply Mem.alloc_glob_result in ALLOC.
+        subst. congruence.
+        erewrite <- store_init_data_list_perm. 2: eapply Heqo0.
+        erewrite <- Genv.store_zeros_perm. 2: eapply Heqo.          
+        eapply Mem.perm_alloc_glob_1 in ALLOC. eapply ALLOC.
+        eauto.
+        congruence.
+        (* 2 *)
+        split.
+        intros.
+        assert (Mem.perm m0 (Global id) ofs k p).
+        eapply Mem.perm_alloc_glob_1 in ALLOC. eapply ALLOC.
+        eapply Genv.store_zeros_perm;eauto.
+        eapply store_init_data_list_perm;eauto.
+        eapply Mem.perm_drop_4;eauto.
+        congruence. eapply P2 in H3.
+        eauto.
+        (* 3 *)
+        split.
+        eapply load_store_init_data_invariant.
+        2: eapply P3. intros.
+        erewrite (Mem.load_drop m3);eauto.
+        erewrite <- store_init_data_list_load_other.
+        2: eapply Heqo0.
+        erewrite <- (Genv.store_zeros_load_other m1);eauto.
+        erewrite Mem.load_alloc_glob_unchanged;eauto.
+        congruence.
+        eapply Mem.alloc_glob_result in ALLOC. subst.
+        congruence.
+        eapply Mem.alloc_glob_result in ALLOC. subst.
+        congruence. 
+        left.
+        eapply Mem.alloc_glob_result in ALLOC.
+        subst. congruence.
+        (* 4 *)
+        erewrite Mem.loadbytes_drop. 2: eapply DROP.
+        erewrite <- store_init_data_list_loadbytes_other.
+        2: eapply Heqo0.
+        erewrite <- Genv.store_zeros_loadbytes_other.
+        2: eapply Heqo.        
+        erewrite Mem.loadbytes_alloc_glob_unchanged.
+        2: eapply ALLOC.
+        congruence. congruence. 
+        eapply Mem.alloc_glob_result in ALLOC.
+        subst. congruence.
+        eapply Mem.alloc_glob_result in ALLOC.
+        subst. congruence.
+        left.
+        eapply Mem.alloc_glob_result in ALLOC.
+        subst. congruence.
+      - destruct H0 as (P1 & P2 & P3 & P4).
+        split.
+        (* 1 *)
+        unfold Mem.range_perm in *.
+        intros.
+        eapply Mem.perm_drop_3;eauto.
+        left. eapply Mem.alloc_glob_result in ALLOC.
+        subst. congruence.
+        erewrite <- store_init_data_list_perm. 2: eapply Heqo0.
+        erewrite <- Genv.store_zeros_perm. 2: eapply Heqo.          
+        eapply Mem.perm_alloc_glob_1 in ALLOC. eapply ALLOC.
+        eauto.
+        congruence.
+        (* 2 *)
+        split.
+        intros.
+        assert (Mem.perm m0 (Global id) ofs k p).
+        eapply Mem.perm_alloc_glob_1 in ALLOC. eapply ALLOC.
+        eapply Genv.store_zeros_perm;eauto.
+        eapply store_init_data_list_perm;eauto.
+        eapply Mem.perm_drop_4;eauto.
+        congruence. eapply P2 in H3.
+        eauto.
+        (* 3 *)
+        split.
+        eapply load_store_init_data_invariant.
+        2: eapply P3. intros.
+        erewrite (Mem.load_drop m3);eauto.
+        erewrite <- store_init_data_list_load_other.
+        2: eapply Heqo0.
+        erewrite <- (Genv.store_zeros_load_other m1);eauto.
+        erewrite Mem.load_alloc_glob_unchanged;eauto.
+        congruence.
+        eapply Mem.alloc_glob_result in ALLOC. subst.
+        congruence.
+        eapply Mem.alloc_glob_result in ALLOC. subst.
+        congruence. 
+        left.
+        eapply Mem.alloc_glob_result in ALLOC.
+        subst. congruence.
+        (* 4 *)
+        erewrite Mem.loadbytes_drop. 2: eapply DROP.
+        erewrite <- store_init_data_list_loadbytes_other.
+        2: eapply Heqo0.
+        erewrite <- Genv.store_zeros_loadbytes_other.
+        2: eapply Heqo.        
+        erewrite Mem.loadbytes_alloc_glob_unchanged.
+        2: eapply ALLOC.
+        congruence. congruence. 
+        eapply Mem.alloc_glob_result in ALLOC.
+        subst. congruence.
+        eapply Mem.alloc_glob_result in ALLOC.
+        subst. congruence.
+        left.
+        eapply Mem.alloc_glob_result in ALLOC.
+        subst. congruence. }
+    eapply IHsecs;eauto.
+Qed.        
+    
+
+    
+Lemma alloc_section_characterization: forall sec id m0 m ge,
+    alloc_section ge (Some m0) id sec = Some m ->
+    globals_initialized_sections ge m (Global id) sec.
+Proof.
+  unfold alloc_section.
+  intros.
+  unfold globals_initialized_sections.
+  destr;simpl in *.
+  - destruct (Mem.alloc_glob id m0 0 (Z.max (code_size instr_size code) 1)) eqn:ALLOC.
+    split.
+    eapply Mem.alloc_glob_result in ALLOC.
+    subst.
+    eapply Mem.perm_drop_1;eauto.
+    lia.
+    intros.
+    exploit Mem.alloc_glob_result;eauto. intro. subst.
+    exploit Mem.perm_drop_4; eauto.
+    intro. exploit Mem.perm_alloc_glob_2; eauto.
+    intros. eapply H2 in H1. split.
+    eauto. eapply Mem.perm_drop_2 in H0;eauto.
+    inv H0;auto.
+  (* writable *)
+  - destruct ( Mem.alloc_glob id m0 0 (init_data_list_size init)) eqn:FOLD.
+    destr_in H.
+    destr_in H.
+    exploit Mem.alloc_glob_result;eauto. intros. subst.
+    split.
+    (* 1 *)
+    unfold Mem.range_perm. intros.
+    eapply Mem.perm_drop_1;eauto.
+    (* 2 *)
+    split. intros.
+    assert (0 <= ofs < init_data_list_size init).
+    exploit Mem.perm_drop_4; eauto.
+    intro. exploit Mem.perm_alloc_glob_2; eauto.
+    intros. exploit Genv.store_zeros_perm;eauto.
+    exploit store_init_data_list_perm;eauto. intros.
+    eapply H3 in H1. eapply H4 in H1.
+    eapply H2. eauto.
+    eapply Mem.perm_drop_2 in H;eauto.
+
+    (* 3 *)
+    split.
+    
+    
+    eapply load_store_init_data_invariant. intros.
+    eapply Mem.load_drop;eauto. repeat right. constructor.
+    
+    eapply store_init_data_list_charact;eauto.
+    (* 4 *)
+    erewrite Mem.loadbytes_drop;eauto.
+    eapply store_init_data_list_loadbytes;eauto.
+    repeat right. constructor.
+    
+  (* readable *)
+  - destruct ( Mem.alloc_glob id m0 0 (init_data_list_size init)) eqn:FOLD.
+    destr_in H.
+    destr_in H.
+    exploit Mem.alloc_glob_result;eauto. intros. subst.
+    split.
+    (* 1 *)
+    unfold Mem.range_perm. intros.
+    eapply Mem.perm_drop_1;eauto.
+    (* 2 *)
+    split. intros.
+    assert (0 <= ofs < init_data_list_size init).
+    exploit Mem.perm_drop_4; eauto.
+    intro. exploit Mem.perm_alloc_glob_2; eauto.
+    intros. exploit Genv.store_zeros_perm;eauto.
+    exploit store_init_data_list_perm;eauto. intros.
+    eapply H3 in H1. eapply H4 in H1.
+    eapply H2. eauto.
+    eapply Mem.perm_drop_2 in H;eauto.
+
+    (* 3 *)
+    split.
+    
+    
+    eapply load_store_init_data_invariant. intros.
+    eapply Mem.load_drop;eauto. repeat right. constructor.
+    
+    eapply store_init_data_list_charact;eauto.
+    (* 4 *)
+    erewrite Mem.loadbytes_drop;eauto.
+    eapply store_init_data_list_loadbytes;eauto.
+    repeat right. constructor.
+Qed.    
+    
+    
+Lemma alloc_external_symbols_none: forall l,
+    fold_left (fun (a : option mem) (p : positive * symbentry) => alloc_external_comm_symbol a (fst p) (snd p))
+              l None = None.
+Proof.
+  induction l;simpl;auto.
+Qed.
+
+Lemma alloc_external_symbols_pres_characterization: forall m0 symbtbl sectbl m ge id sec,
+    sectbl!id = Some sec ->
+    well_formed_symbtbl sectbl symbtbl ->
+    alloc_external_symbols m0 symbtbl = Some m ->
+    globals_initialized_sections ge m0 (Global id) sec ->
+    globals_initialized_sections ge m (Global id) sec.
+Proof.
+  unfold well_formed_symbtbl,alloc_external_symbols.
+  intros m0 symbtbl sectbl m ge id sec G W ALLOC P.
+  assert (WF: forall (id : positive) (e : symbentry),
+       In (id,e) (PTree.elements symbtbl) ->
+       match symbentry_secindex e with
+       | secindex_normal i =>
+           symbentry_type e <> symb_notype /\
+           i = id /\
+           (exists sec : RelocProg.section instruction init_data,
+              sectbl ! i = Some sec /\ sec_size instr_size sec = symbentry_size e /\ symbentry_value e = 0)
+       | secindex_comm => symbentry_type e = symb_data /\ sectbl ! id = None
+       | secindex_undef => symbentry_type e <> symb_notype /\ sectbl ! id = None
+       end).
+  intros. eapply W. eapply PTree.elements_complete. auto.
+  clear W.
+
+  rewrite PTree.fold_spec in ALLOC.
+  set (l:= (PTree.elements symbtbl)) in *.
+  generalize l m m0 WF ALLOC P. clear l m m0 WF ALLOC P.
+  induction l;simpl. intros.
+  inv ALLOC. auto.
+  
+  intros.
+
+  (* we should ensure ALLOC return some *)
+  destruct a;simpl in *.
+
+  exploit WF. left. eauto.
+  intros WF'.
+  
+  destr_in WF'.
+  
+  - destr_in ALLOC. 
+    eapply IHl. 2: eapply ALLOC.
+    intros. eapply WF. auto. auto.
+    eapply IHl. 2: eapply ALLOC.
+    intros. eapply WF. auto. auto.
+  - destruct WF'.
+    rewrite H in *.
+    destruct (Mem.alloc_glob p m0 0 ((Z.max (symbentry_size s) 0))) eqn:GLOB.
+    destr_in ALLOC.
+    destruct ((Mem.drop_perm m2 b 0 (Z.max (symbentry_size s) 0) Writable)) eqn:DROP.
+    eapply IHl. 2: eapply ALLOC.
+    intros. eapply WF. auto.
+    assert (p <> id).
+    unfold not. intros. subst. congruence.
+    exploit Mem.alloc_glob_result;eauto. intros. subst.
+    eapply drop_pres_globals_initialized_sections.
+    eapply store_zeros_pres_globals_initialized_sections.
+    eapply alloc_glob_pres_globals_initialized_sections;eauto.
+    congruence. eauto.
+    congruence. eauto.
+    congruence.
+
+    erewrite alloc_external_symbols_none in ALLOC. congruence.
+    erewrite alloc_external_symbols_none in ALLOC. congruence.
+  - destruct WF'.
+    destr_in ALLOC;try congruence.
+    + destruct (Mem.alloc_glob p m0 0 1) eqn:GLOB.
+      destruct ((Mem.drop_perm m1 b 0 1 Nonempty)) eqn:DROP.
+      eapply IHl. 2: eapply ALLOC.
+      intros. eapply WF. auto.
+      assert (p <> id).
+      unfold not. intros. subst. congruence.
+      exploit Mem.alloc_glob_result;eauto. intros. subst.
+      eapply drop_pres_globals_initialized_sections.
+      eapply alloc_glob_pres_globals_initialized_sections;eauto.
+      congruence. eauto.
+      congruence.
+      
+      erewrite alloc_external_symbols_none in ALLOC. congruence.
+    + destruct (Mem.alloc_glob p m0 0 1) eqn:GLOB.
+      destr_in ALLOC.
+      destruct ((Mem.drop_perm m2 b 0 1 Nonempty)) eqn:DROP.
+      eapply IHl. 2: eapply ALLOC.
+      intros. eapply WF. auto.
+      assert (p <> id).
+      unfold not. intros. subst. congruence.
+      exploit Mem.alloc_glob_result;eauto. intros. subst.
+      eapply drop_pres_globals_initialized_sections.
+      eapply store_zeros_pres_globals_initialized_sections.
+      eapply alloc_glob_pres_globals_initialized_sections;eauto.
+      congruence. eauto.
+      congruence. eauto.
+      congruence.
+      erewrite alloc_external_symbols_none in ALLOC. congruence.
+      erewrite alloc_external_symbols_none in ALLOC. congruence.
+Qed.
+
+
+Lemma alloc_external_symbols_pres_external_characterization: 
+  forall symbs symb ge m0 m id,
+    ~ In id (map fst symbs) ->
+    globals_initialized_external ge m0 (Global id) symb ->
+    fold_left (fun (a : option mem) (p : positive * symbentry) => alloc_external_comm_symbol a (fst p) (snd p))
+              symbs (Some m0) = Some m ->
+    globals_initialized_external ge m (Global id) symb.
+Proof.
+  induction symbs;simpl;intros.
+  inv H1. auto.
+  destruct a;simpl in *.
+  eapply Decidable.not_or in H.
+  destruct H.
+
+  rename H1 into ALLOC.
+  destr_in ALLOC.
+  - destr_in ALLOC.
+    + eapply IHsymbs;eauto.
+    + erewrite alloc_external_symbols_none in ALLOC. congruence.
+    + destruct (Mem.alloc_glob i m0 0 1) eqn:GLOB.      
+      destruct ((Mem.drop_perm m1 b 0 1 Nonempty)) eqn:DROP.
+      eapply IHsymbs. 3: eapply ALLOC. auto.
+      exploit Mem.alloc_glob_result;eauto. intros. subst.
+      eapply drop_pres_globals_initialized_external.
+      eapply alloc_glob_pres_globals_initialized_external;eauto.
+      congruence. eauto.
+      congruence. eauto.
+      
+      erewrite alloc_external_symbols_none in ALLOC. congruence.
+  - destr_in ALLOC.
+    + eapply IHsymbs;eauto.
+    + destruct (Mem.alloc_glob i m0 0 (Z.max (symbentry_size s) 0)) eqn:GLOB.
+      destr_in ALLOC.
+      destruct ((Mem.drop_perm m2 b 0 (Z.max (symbentry_size s) 0) Writable)) eqn:DROP.
+      eapply IHsymbs. 3: eapply ALLOC. auto.
+      exploit Mem.alloc_glob_result;eauto. intros. subst.
+      eapply drop_pres_globals_initialized_external.
+      eapply store_zeros_pres_globals_initialized_external.
+      eapply alloc_glob_pres_globals_initialized_external;eauto.
+      congruence. eauto.
+      congruence. eauto.
+      congruence.
+      erewrite alloc_external_symbols_none in ALLOC. congruence.
+      erewrite alloc_external_symbols_none in ALLOC. congruence.
+    + destruct (Mem.alloc_glob i m0 0 1) eqn:GLOB.
+      destr_in ALLOC.
+      destruct ((Mem.drop_perm m2 b 0 1 Nonempty)) eqn:DROP.
+      eapply IHsymbs. 3: eapply ALLOC. auto.
+      exploit Mem.alloc_glob_result;eauto. intros. subst.
+      eapply drop_pres_globals_initialized_external.
+      eapply store_zeros_pres_globals_initialized_external.
+      eapply alloc_glob_pres_globals_initialized_external;eauto.
+      congruence. eauto.
+      congruence. eauto.
+      congruence.
+      erewrite alloc_external_symbols_none in ALLOC. congruence.
+      erewrite alloc_external_symbols_none in ALLOC. congruence.
+
+  - erewrite alloc_external_symbols_none in ALLOC. congruence.
+Qed.
+
+Lemma alloc_external_characterization: forall symb id m0 m ge ,
+    symbentry_secindex symb = secindex_comm \/ symbentry_secindex symb = secindex_undef ->
+    alloc_external_comm_symbol (Some m0) id symb = Some m ->
+    globals_initialized_external ge m (Global id) symb.
+Proof.
+  unfold alloc_external_comm_symbol, globals_initialized_external.
+  intros.
+  rename H0 into ALLOC.
+  destruct H;rewrite H in *.
+  - destr.
+    + destruct (Mem.alloc_glob id m0 0 (Z.max (symbentry_size symb) 0)) eqn:GLOB.
+      destr_in ALLOC.
+      exploit Mem.alloc_glob_result;eauto. intros. subst.
+      split.
+      (* 1 *)
+      unfold Mem.range_perm. intros.
+      eapply Mem.perm_drop_1;eauto.
+      (* 2 *)
+      split. intros.
+      assert (0 <= ofs < Z.max (symbentry_size symb) 0).
+      exploit Mem.perm_drop_4; eauto.
+      intro. exploit Mem.perm_alloc_glob_2; eauto.
+      intros. exploit Genv.store_zeros_perm;eauto.
+      intros.
+      eapply H3 in H1. eapply H2 in H1.
+      auto.
+      split. auto.
+      eapply Mem.perm_drop_2 in ALLOC;eauto.
+      
+      (* 3 *)
+      split.          
+      eapply load_store_init_data_invariant. intros.
+      eapply Mem.load_drop;eauto. repeat right. constructor.
+      simpl. split;auto.
+
+      eapply Genv.store_zeros_read_as_zero;eauto.
+      (* rewrite store_zeros_equation in *. destr_in Heqo. *)
+
+      (* assert ((Z.max (symbentry_size symb) 0) = 0). lia. *)
+      (* rewrite H0. rewrite zle_true. eapply Heqo. lia. *)
+      (* assert (Z.max (symbentry_size symb) 0 = (symbentry_size symb)) by lia. *)
+      (* destr. rewrite H0. auto. *)
+
+      (* 4 *)
+      erewrite Mem.loadbytes_drop;eauto.
+      simpl.
+
+      
+      generalize (Genv.store_zeros_loadbytes _ _ _ Heqo).
+      unfold Genv.readbytes_as_zero. intros. rewrite app_nil_r.
+      rewrite <- Z_to_nat_max.
+      
+      eapply H0.
+      lia. lia.
+
+      repeat right. constructor.
+      
+  - destr.  
+    + destruct (Mem.alloc_glob id m0 0 1) eqn:GLOB.
+      exploit Mem.alloc_glob_result;eauto;intros;subst.
+      split.
+      * eapply Mem.perm_drop_1;eauto. lia.
+      * intros. exploit Mem.perm_drop_4; eauto.
+        intro. exploit Mem.perm_alloc_glob_2; eauto.
+        intros. eapply H2 in H1. split.
+        lia. eapply Mem.perm_drop_2 in H0;eauto.
+        inv H0;auto.
+    + destruct (Mem.alloc_glob id m0 0 1) eqn:GLOB.
+      destr_in ALLOC.
+      exploit Mem.alloc_glob_result;eauto;intros;subst.
+      split.
+      * eapply Mem.perm_drop_1;eauto. lia.
+      * intros. exploit Mem.perm_drop_4; eauto.
+        intro. exploit Mem.perm_alloc_glob_2; eauto.
+        intros.
+        exploit Genv.store_zeros_perm;eauto. intros.
+        eapply H3 in H1. eapply H2 in H1. split.
+        lia. eapply Mem.perm_drop_2 in H0;eauto.
+        inv H0;auto.
+Qed.    
+
+(** Properties about init_mem *)
+Lemma init_mem_characterization_gen: forall p m,
+    well_formed_symbtbl (prog_sectable p) (prog_symbtable p) ->
+    init_mem p = Some m ->
+    globals_initialized (globalenv p) p m.
+Proof.
+   unfold init_mem.
+   unfold globals_initialized.
+   intros p m WF H id b ofs0 G. destr_in H.
+   
+   (* symbentry exists *)
+   unfold globalenv in G. unfold Genv.find_symbol in G.
+   unfold gen_symb_map in G.
+   simpl in G. rewrite PTree.gmap in G. unfold option_map in G.
+   destr_in G.
+
+   unfold well_formed_symbtbl in WF.
+   generalize (WF id s Heqo0). rename WF into WF0. intros WF.
+   unfold gen_global in G.
+   (* destruct symbentry_secindex s *)
+   
+   generalize (PTree.elements_keys_norepet (prog_sectable p)).
+   generalize (PTree.elements_keys_norepet (prog_symbtable p)).
+   intros NOREP1 NOREP2.
+   
+   destruct (symbentry_secindex s) eqn:SECIDX.
+   - inv G. 
+     destruct WF as (P1 & P2 & sec & P3 & P4 & P5).
+     rewrite P5. rewrite Ptrofs.unsigned_repr. simpl.
+     subst. rewrite P3.
+     2: { unfold Ptrofs.max_unsigned. unfold Ptrofs.modulus.
+          unfold Ptrofs.wordsize. unfold Wordsize_Ptrofs.wordsize.
+          destr;simpl;lia. }
+     
+     unfold alloc_sections in Heqo. rewrite PTree.fold_spec in Heqo.
+     exploit PTree.elements_correct;eauto. 
+     intros INELE.
+     unfold section in *.
+     set (l:= (PTree.elements (prog_sectable p))) in *.
+     eapply in_norepet_unique in INELE;eauto. destruct INELE as (gl1 & gl2 & Q1 & Q2 & Q3).
+     rewrite Q1 in *.
+     rewrite fold_left_app in Heqo.
+     simpl in Heqo.
+     unfold ident in *.
+     set (m0':=(fold_left
+                  (fun (a : option mem) (p0 : positive * RelocProg.section instruction init_data) =>
+                     alloc_section (globalenv p) a (fst p0) (snd p0)) gl1 (Some Mem.empty))) in Heqo.
+     destruct m0'.
+     + destruct ((alloc_section (globalenv p) (Some m1) id sec)) eqn:ALLOC.
+       * eapply alloc_section_characterization in ALLOC.
+         exploit alloc_sections_pres_characterization. eapply Q2.
+         eapply ALLOC. eauto.
+         intros Q.
+         exploit alloc_external_symbols_pres_characterization;eauto.
+       * erewrite alloc_sections_none in Heqo.
+         congruence.
+     + simpl in Heqo.
+       erewrite alloc_sections_none in Heqo.
+       congruence.
+   - destruct WF as (P1 & P2).
+     rewrite P2. rewrite P1.
+     inv G. 
+     unfold alloc_external_symbols in H. rewrite PTree.fold_spec in H.
+     exploit PTree.elements_correct;eauto. 
+     intros INELE.
+     unfold section in *.
+     set (l:= (PTree.elements (prog_symbtable p))) in *.
+     eapply in_norepet_unique in INELE;eauto. destruct INELE as (gl1 & gl2 & Q1 & Q2 & Q3).
+     rewrite Q1 in *.
+     rewrite fold_left_app in H.
+     simpl in H.
+     unfold ident in *.
+     set (m0':=(fold_left
+           (fun (a : option mem) (p : positive * symbentry) => alloc_external_comm_symbol a (fst p) (snd p)) gl1
+           (Some m0))) in *.
+     destruct m0'.
+     + destruct (alloc_external_comm_symbol (Some m1) id s) eqn:ALLOC.
+       * eapply alloc_external_characterization in ALLOC.
+         exploit alloc_external_symbols_pres_external_characterization. eapply Q2.
+         eapply ALLOC. eauto.
+         unfold globals_initialized_external.
+         rewrite P1. rewrite SECIDX.
+         eauto. auto.
+       * erewrite alloc_external_symbols_none in H.
+         congruence.
+     + simpl in H.
+       erewrite alloc_external_symbols_none in H.
+       congruence.
+   - destruct WF as (P1 & P2).
+     rewrite P2. destr.
+     (* 2 same goals *)
+     { inv G. 
+     unfold alloc_external_symbols in H. rewrite PTree.fold_spec in H.
+     exploit PTree.elements_correct;eauto. 
+     intros INELE.
+     unfold section in *.
+     set (l:= (PTree.elements (prog_symbtable p))) in *.
+     eapply in_norepet_unique in INELE;eauto. destruct INELE as (gl1 & gl2 & Q1 & Q2 & Q3).
+     rewrite Q1 in *.
+     rewrite fold_left_app in H.
+     simpl in H.
+     unfold ident in *.
+     set (m0':=(fold_left
+           (fun (a : option mem) (p : positive * symbentry) => alloc_external_comm_symbol a (fst p) (snd p)) gl1
+           (Some m0))) in *.
+     destruct m0'.
+     + destruct (alloc_external_comm_symbol (Some m1) id s) eqn:ALLOC.
+       * eapply alloc_external_characterization in ALLOC.
+         generalize (alloc_external_symbols_pres_external_characterization gl2 s (globalenv p) m2 m id Q2 ALLOC H). 
+         unfold globals_initialized_external.
+         rewrite Heqs0. rewrite SECIDX.
+         eauto. auto.
+       * erewrite alloc_external_symbols_none in H.
+         congruence.
+     + simpl in H.
+       erewrite alloc_external_symbols_none in H.
+       congruence. }
+
+     inv G.
+     unfold alloc_external_symbols in H. rewrite PTree.fold_spec in H.
+     exploit PTree.elements_correct;eauto. 
+     intros INELE.
+     unfold section in *.
+     set (l:= (PTree.elements (prog_symbtable p))) in *.
+     eapply in_norepet_unique in INELE;eauto. destruct INELE as (gl1 & gl2 & Q1 & Q2 & Q3).
+     rewrite Q1 in *.
+     rewrite fold_left_app in H.
+     simpl in H.
+     unfold ident in *.
+     set (m0':=(fold_left
+           (fun (a : option mem) (p : positive * symbentry) => alloc_external_comm_symbol a (fst p) (snd p)) gl1
+           (Some m0))) in *.
+     destruct m0'.
+     + destruct (alloc_external_comm_symbol (Some m1) id s) eqn:ALLOC.
+       * eapply alloc_external_characterization in ALLOC.
+         generalize (alloc_external_symbols_pres_external_characterization gl2 s (globalenv p) m2 m id Q2 ALLOC H). 
+         unfold globals_initialized_external.
+         rewrite Heqs0. rewrite SECIDX.
+         eauto. auto.
+       * erewrite alloc_external_symbols_none in H.
+         congruence.
+     + simpl in H.
+       erewrite alloc_external_symbols_none in H.
+       congruence.
+Qed.       
+
+
+
+(** Some properties of initialization of data  *)
+Lemma store_init_data_nextblock: forall v ge m b ofs m',
+  store_init_data ge m b ofs v = Some m' ->
+  Mem.nextblock m' = Mem.nextblock m.
+
+         
+Proof.
+  intros. destruct v; simpl in *; try now (eapply Mem.nextblock_store; eauto).
+  eapply Genv.store_zeros_nextblock.
+  eauto.
+
+  (* destr_in H. destruct p. eapply Mem.nextblock_store;eauto. *)
+  
+Qed.
+    
+Lemma store_init_data_list_nextblock: forall l ge m b ofs m',
+  store_init_data_list ge m b ofs l = Some m' ->
+  Mem.nextblock m' = Mem.nextblock m.
+ Proof.
+  induction l; intros.
+  - inv H. auto.
+  - inv H. destr_match_in H1; inv H1.
+    exploit store_init_data_nextblock; eauto.
+    exploit IHl; eauto. intros. congruence.
+Qed.
+
+Lemma store_init_data_list_support: forall l ge m b ofs m',
+    store_init_data_list ge m b ofs l = Some m' ->
+    Mem.support m' = Mem.support m.
+Proof.
+  induction l;intros.
+  - inv H. auto.
+  - inv H. destr_match_in H1;inv H1.
+    transitivity (Mem.support m0). eapply IHl. eauto.
+    destruct a;simpl in EQ;try (eapply Mem.support_store;eauto;fail).
+    eapply Genv.store_zeros_support. eauto.
+
+    (* destr_in EQ. destruct p. eapply Mem.support_store;eauto. *)
+Qed.
+
+Lemma store_init_data_stack : forall v ge (m m' : mem) (b : block) (ofs : Z),
+       store_init_data ge m b ofs v = Some  m' -> Mem.stack (Mem.support m') = Mem.stack (Mem.support m).
+Proof.
+  intros v ge0 m m' b ofs H. destruct v; simpl in *;try (f_equal;now eapply Mem.support_store; eauto).
+  eapply Genv.store_zeros_stack.
+  eauto.
+
+  (* destr_in H. destruct p. f_equal;eapply Mem.support_store; eauto. *)
+Qed.
+
+Lemma store_init_data_list_stack : forall l ge (m m' : mem) (b : block) (ofs : Z),
+       store_init_data_list ge m b ofs l = Some m' -> Mem.stack (Mem.support m') = Mem.stack (Mem.support m).
+Proof.
+  induction l; intros.
+  - simpl in H. inv H. auto.
+  - simpl in H. destr_match_in H; inv H.
+    exploit store_init_data_stack; eauto.
+    exploit IHl; eauto.
+    intros. congruence.
+Qed.
+
+Lemma alloc_section_stack: forall ge id sec m m',
+    alloc_section ge (Some m) id sec = Some m' ->
+    Mem.stack (Mem.support m) = Mem.stack (Mem.support m').
+Proof.
+  unfold alloc_section. intros.
+  repeat destr_in H.
+  exploit Mem.support_drop;eauto.
+  exploit Mem.support_alloc_glob;eauto. intros.
+  rewrite H0. rewrite H. auto.
+  exploit Mem.support_drop;eauto.
+  exploit Mem.support_alloc_glob;eauto. intros.
+  exploit Genv.store_zeros_stack;eauto. intros (?&?).
+  exploit store_init_data_list_stack;eauto. intros.
+  rewrite H0. rewrite H4. rewrite H2.
+  rewrite H. auto.
+  exploit Mem.support_drop;eauto.
+  exploit Mem.support_alloc_glob;eauto. intros.
+  exploit Genv.store_zeros_stack;eauto. intros (?&?).
+  exploit store_init_data_list_stack;eauto. intros.
+  rewrite H0. rewrite H4. rewrite H2.
+  rewrite H. auto.
+Qed.  
+
+Definition alloc_property_aux (m: mem) (optm': option mem):=
+  forall m', optm' = Some m' ->
+        Mem.stack (Mem.support m) = Mem.stack (Mem.support m').
+
+Lemma alloc_sections_stack_aux: forall ge defs m,
+     alloc_property_aux m
+            (fold_left
+    (fun (a : option mem) (p : positive * section) =>
+     alloc_section ge a (fst p) (snd p))
+    defs (Some m)).
+Proof.
+  intros. eapply Bounds.fold_left_preserves.
+  unfold alloc_property_aux. intros.
+  destruct a.
+  eapply alloc_section_stack in H0. rewrite <- H0.
+  eapply H. auto.
+  simpl in H0. inv H0.
+  unfold alloc_property_aux. intros. inv H. auto.
+Qed.
+  
+Lemma alloc_sections_stack: forall ge sectbl m m',
+    alloc_sections ge sectbl m = Some m' ->
+    Mem.stack (Mem.support m) = Mem.stack (Mem.support m').
+Proof.
+  
+  unfold alloc_sections. intros ge sectbl m m'.
+  rewrite PTree.fold_spec. intros.
+  exploit alloc_sections_stack_aux;eauto.
+Qed.
+
+Lemma alloc_external_symbol_stack: forall id e m m',
+    alloc_external_comm_symbol(Some m) id e = Some m' ->
+    Mem.stack (Mem.support m) = Mem.stack (Mem.support m').
+Proof.
+  unfold alloc_external_comm_symbol.
+  intros. repeat destr_in H.
+  exploit Mem.support_drop;eauto.
+  exploit Mem.support_alloc_glob;eauto. intros.
+  rewrite H0. rewrite H. auto.
+  exploit Mem.support_drop;eauto.
+  exploit Mem.support_alloc_glob;eauto. intros.
+  exploit Genv.store_zeros_stack;eauto. intros (?&?).
+  rewrite H0. rewrite H2. rewrite H. auto.
+  exploit Mem.support_drop;eauto.
+  exploit Mem.support_alloc_glob;eauto. intros.
+  exploit Genv.store_zeros_stack;eauto. intros (?&?).
+  rewrite H0. rewrite H2. rewrite H. auto.
+  (* exploit Mem.support_drop;eauto. *)
+  (* exploit Mem.support_alloc_glob;eauto. intros. *)
+  (* exploit Genv.store_zeros_stack;eauto. intros (?&?). *)
+  (* rewrite H0. rewrite H2. rewrite H. auto. *)
+  (* exploit Mem.support_drop;eauto. *)
+  (* exploit Mem.support_alloc_glob;eauto. intros. *)
+  (* exploit Genv.store_zeros_stack;eauto. intros (?&?). *)
+  (* rewrite H0. rewrite H2. rewrite H. auto. *)
+Qed.
+
+
+
+Lemma alloc_external_symbols_stack: forall symbtbl m m',
+    alloc_external_symbols m symbtbl = Some m' ->
+    Mem.stack (Mem.support m) = Mem.stack (Mem.support m').
+Proof.
+  unfold alloc_external_symbols. intros.
+  rewrite PTree.fold_spec in H.
+  assert (alloc_property_aux m (fold_left
+        (fun (a : option mem) (p : positive * symbentry) =>
+         alloc_external_comm_symbol a (fst p) (snd p))
+        (PTree.elements symbtbl) (Some m))).
+  eapply Bounds.fold_left_preserves.
+  unfold alloc_property_aux.
+  intros.
+  destruct a.
+  eapply alloc_external_symbol_stack in H1.
+  rewrite <- H1.  eapply H0. auto.
+  simpl in H1. congruence.
+  unfold alloc_property_aux.
+  intros. inv H0;auto.
+  unfold alloc_property_aux in H0.
+  eapply H0. auto.
+Qed.
+
+
+Lemma init_mem_stack:
+  forall p m,
+    init_mem p = Some m ->
+    Mem.stack (Mem.support m) = Node None nil nil None.
+Proof.
+  intros. unfold init_mem in H.
+  repeat destr_in H.
+  erewrite <- alloc_external_symbols_stack; eauto.
+  erewrite <- alloc_sections_stack; eauto.
+  simpl. auto.
+Qed.
+
+Section STORE_INIT_DATA_PRESERVED.
+  Variable ge1: Genv.t.
+  Variable ge2: Genv.t.
+
+  Hypothesis symbols_preserved:
+    forall id, Genv.find_symbol ge2 id = Genv.find_symbol ge1 id.
+
+  Lemma store_init_data_pres: forall d m b ofs,
+      store_init_data ge1 m b ofs d = store_init_data ge2 m b ofs d.
+  Proof.
+    destruct d;simpl;auto.
+    intros.
+    assert (EQ: forall id ofs, Genv.symbol_address ge2 id ofs = Genv.symbol_address ge1 id ofs).
+    { unfold Genv.symbol_address; simpl; intros. rewrite symbols_preserved;auto. }
+    (* rewrite symbols_preserved. *)
+    rewrite EQ.
+    auto.
+  Qed.
+
+  Lemma store_init_data_list_pres: forall l m b ofs,
+      store_init_data_list ge1 m b ofs l = store_init_data_list ge2 m b ofs l.
+  Proof.
+    induction l;auto.
+    intros. simpl. rewrite store_init_data_pres.
+    destr.
+  Qed.
+  
+End STORE_INIT_DATA_PRESERVED.
+
+(* Some properties of allocation *)
+
+Lemma alloc_sections_valid_aux: forall l b m m' ge,
+    fold_left
+      (fun (a : option mem)
+         (p : positive * RelocProg.section instruction init_data)
+       => alloc_section ge a (fst p) (snd p)) l (Some m) = Some m' ->
+      sup_In b m.(Mem.support) ->
+      sup_In b m'.(Mem.support).
+Proof.
+  induction l;intros.
+  simpl in H. inv H. auto.
+  simpl in H. destruct a.
+  destruct s.
+  - simpl in *.
+    destruct Mem.alloc_glob eqn:ALLOC in H.
+    apply Mem.support_alloc_glob in ALLOC.
+    destruct (Mem.drop_perm) eqn:FOLD in H.
+    eapply IHl;eauto.
+    eapply Mem.drop_perm_valid_block_1;eauto.
+    unfold Mem.valid_block.
+    rewrite ALLOC.
+    apply Mem.sup_incr_glob_in. right. auto.
+    clear IHl.
+    induction l;simpl in H.
+    inv H.  apply IHl. auto.
+  - simpl in *.
+    destruct Mem.alloc_glob eqn:ALLOC in H.
+    destr_in H. destr_in H.
+    apply Mem.support_alloc_glob in ALLOC.
+    destruct (Mem.drop_perm) eqn:FOLD in H.
+    eapply IHl;eauto.
+    eapply Mem.drop_perm_valid_block_1;eauto.
+    unfold Mem.valid_block.
+    
+    eapply store_init_data_list_support in Heqo0.
+    rewrite Heqo0.
+    eapply Genv.store_zeros_support in Heqo. rewrite Heqo.
+    rewrite ALLOC.
+    apply Mem.sup_incr_glob_in. right. auto.
+    clear IHl.
+    induction l;simpl in H.
+    inv H.  apply IHl. auto.
+    clear IHl.
+    induction l;simpl in H.
+    inv H.  apply IHl. auto.
+        clear IHl.
+    induction l;simpl in H.
+    inv H.  apply IHl. auto.
+
+  - simpl in *.
+    destruct Mem.alloc_glob eqn:ALLOC in H.
+    destr_in H. destr_in H.
+    apply Mem.support_alloc_glob in ALLOC.
+    destruct (Mem.drop_perm) eqn:FOLD in H.
+    eapply IHl;eauto.
+    eapply Mem.drop_perm_valid_block_1;eauto.
+    unfold Mem.valid_block.
+    
+    eapply store_init_data_list_support in Heqo0.
+    rewrite Heqo0.
+    eapply Genv.store_zeros_support in Heqo. rewrite Heqo.
+    rewrite ALLOC.
+    apply Mem.sup_incr_glob_in. right. auto.
+    clear IHl.
+    induction l;simpl in H.
+    inv H.  apply IHl. auto.
+    clear IHl.
+    induction l;simpl in H.
+    inv H.  apply IHl. auto.
+        clear IHl.
+    induction l;simpl in H.
+    inv H.  apply IHl. auto.
+Qed.
+
+
+Remark in_norepet_unique_r:
+  forall T (gl: list (ident * T)) id g,
+  In (id, g) gl -> list_norepet (map fst gl) ->
+  exists gl1 gl2, gl = gl1 ++ (id, g) :: gl2 /\ ~In id (map fst gl2).
+Proof.
+  induction gl as [|[id1 g1] gl]; simpl; intros.
+  contradiction.
+  inv H0. destruct H.
+  inv H. exists nil, gl. auto.
+  exploit IHgl; eauto. intros (gl1 & gl2 & X & Y).
+  exists ((id1, g1) :: gl1), gl2; split;auto. rewrite X; auto.
+Qed.
+
+
+Lemma alloc_sections_valid: forall id sec sectbl m m' ge,
+      sectbl ! id = Some sec ->
+      alloc_sections ge sectbl m = Some m' ->     
+      sup_In (Global id) m'.(Mem.support).
+Proof.
+  unfold alloc_sections.
+  intros id sec sectbl m m' ge A1 A2 .
+  rewrite PTree.fold_spec in A2.
+  apply PTree.elements_correct in A1.
+  generalize (PTree.elements_keys_norepet sectbl).
+  intros NOREP.
+  exploit in_norepet_unique_r;eauto.
+  intros (gl1 & gl2 & P1 & P2).
+  unfold section in *. rewrite P1 in *.
+  rewrite fold_left_app in A2.
+  simpl in A2.
+   unfold ident in *.
+  destruct ((alloc_section ge
+            (fold_left
+               (fun (a : option mem)
+                  (p : positive *
+                       RelocProg.section instruction init_data) =>
+                alloc_section ge a (fst p) (snd p)) gl1 
+               (Some m)) id sec)) eqn:FOLD.
+  - 
+    exploit alloc_sections_valid_aux;eauto.
+    unfold alloc_section in FOLD at 1. destr_in FOLD.
+    destruct sec.
+    + simpl in *.
+      destruct Mem.alloc_glob eqn:ALLOC in FOLD.
+      apply Mem.support_alloc_glob in ALLOC.
+      generalize (Mem.sup_incr_glob_in1 id (Mem.support m1)).
+      rewrite <- ALLOC.
+      intros.
+      exploit Mem.drop_perm_valid_block_1;eauto.
+    + simpl in *.     
+      destruct Mem.alloc_glob eqn:ALLOC in FOLD.
+      repeat destr_in FOLD.
+      apply Mem.support_alloc_glob in ALLOC.      
+      generalize (Mem.sup_incr_glob_in1 id (Mem.support m1)).
+      rewrite <- ALLOC.
+      exploit Genv.store_zeros_support;eauto.
+      exploit store_init_data_list_support;eauto.
+      intros. rewrite <- H1 in *.
+      rewrite <- H in *.
+      exploit Mem.drop_perm_valid_block_1;eauto.
+    + simpl in *.     
+      destruct Mem.alloc_glob eqn:ALLOC in FOLD.
+      repeat destr_in FOLD.
+      apply Mem.support_alloc_glob in ALLOC.      
+      generalize (Mem.sup_incr_glob_in1 id (Mem.support m1)).
+      rewrite <- ALLOC.
+      exploit Genv.store_zeros_support;eauto.
+      exploit store_init_data_list_support;eauto.
+      intros. rewrite <- H1 in *.
+      rewrite <- H in *.
+      exploit Mem.drop_perm_valid_block_1;eauto.
+  - clear A1 NOREP P1 P2.
+    induction gl2.
+    simpl in A2. inv A2.
+    apply IHgl2. auto.
+Qed.
+
+Lemma alloc_external_symbols_valid_aux2: forall l,
+        fold_left
+          (fun (a : option mem) (p : positive * symbentry) =>
+             alloc_external_comm_symbol a (fst p) (snd p)) l None =
+        None.
+Proof.
+  induction l;simpl;auto.
+Qed.
+
+Lemma alloc_external_symbols_valid_aux: forall l m m' b,
+    fold_left
+      (fun (a : option mem) (p : positive * symbentry) =>
+         alloc_external_comm_symbol a (fst p) (snd p)) l (Some m) =
+    Some m' ->
+    sup_In b (Mem.support m) ->
+    sup_In b (Mem.support m').
+Proof.
+  induction l;intros.
+  simpl in H. inv H. auto.
+  simpl in H.
+  destruct (symbentry_type (snd a)).
+  - destruct (symbentry_secindex (snd a)).
+    + eapply IHl;eauto.
+    + rewrite alloc_external_symbols_valid_aux2 in H. inv H.
+    + destruct Mem.alloc_glob eqn:ALLOC in H.
+      destruct Mem.drop_perm eqn:DROP in H.
+      eapply IHl;eauto.
+      eapply Mem.drop_perm_valid_block_1;eauto.
+      unfold Mem.valid_block. apply Mem.support_alloc_glob in ALLOC.
+      rewrite ALLOC. eapply Mem.sup_incr_glob_in.
+      right. auto.
+      rewrite alloc_external_symbols_valid_aux2 in H. inv H.
+  - destruct (symbentry_secindex (snd a)).
+    + eapply IHl;eauto.
+    + destruct Mem.alloc_glob eqn:ALLOC in H.
+      destruct store_zeros eqn:STORE in H.
+      destruct Mem.drop_perm eqn:DROP in H.
+      eapply IHl;eauto.
+      eapply Mem.drop_perm_valid_block_1;eauto.
+      unfold Mem.valid_block.
+      erewrite Genv.store_zeros_support.
+      apply Mem.support_alloc_glob in ALLOC.
+      rewrite ALLOC. eapply Mem.sup_incr_glob_in.
+      right. auto.  eauto.
+      rewrite alloc_external_symbols_valid_aux2 in H. inv H.
+      rewrite alloc_external_symbols_valid_aux2 in H. inv H.
+    + destruct Mem.alloc_glob eqn:ALLOC in H.
+      destruct store_zeros eqn:STORE in H.
+      destruct Mem.drop_perm eqn:DROP in H.
+      eapply IHl;eauto.
+      eapply Mem.drop_perm_valid_block_1;eauto.
+      unfold Mem.valid_block.
+      erewrite Genv.store_zeros_support.
+      apply Mem.support_alloc_glob in ALLOC.
+      rewrite ALLOC. eapply Mem.sup_incr_glob_in.
+      right. auto.  eauto.
+      rewrite alloc_external_symbols_valid_aux2 in H. inv H.
+      rewrite alloc_external_symbols_valid_aux2 in H. inv H.
+  - rewrite alloc_external_symbols_valid_aux2 in H. inv H.
+Qed.            
+    
+Lemma alloc_external_symbols_valid: forall id e symbtbl m m',
+    symbtbl ! id = Some e ->
+    alloc_external_symbols m symbtbl = Some m' ->
+    match symbentry_secindex e with
+    | secindex_normal i =>
+      sup_In (Global i) m.(Mem.support) ->
+      sup_In (Global i) m'.(Mem.support)
+    | secindex_comm =>
+      symbentry_type e = symb_data ->
+      sup_In (Global id) m'.(Mem.support)
+    | secindex_undef =>
+      symbentry_type e <> symb_notype ->
+      sup_In (Global id) m'.(Mem.support)
+    end.
+Proof.
+  unfold alloc_external_symbols.
+  intros id e symbtbl m m' A1 A2.
+  rewrite PTree.fold_spec in A2.
+  apply PTree.elements_correct in A1.
+  generalize (PTree.elements_keys_norepet symbtbl).
+  intros NOREP.
+  exploit in_norepet_unique_r;eauto.
+  intros (gl1 & gl2 & P1 & P2).
+  rewrite P1 in *.
+  rewrite fold_left_app in A2.
+  simpl in A2.
+  unfold ident in *.
+  destruct (fold_left
+               (fun (a : option mem) (p : positive * symbentry) =>
+                alloc_external_comm_symbol a (fst p) (snd p)) gl1
+               (Some m)) eqn:FOLD.
+  simpl in A2.
+  - destruct (symbentry_secindex e).
+    + destruct (symbentry_type e).
+      * intros.
+        exploit alloc_external_symbols_valid_aux.
+        eapply FOLD. eauto. intros.
+        exploit alloc_external_symbols_valid_aux.
+        eapply A2. eauto. auto.
+      * intros.
+        exploit alloc_external_symbols_valid_aux.
+        eapply FOLD. eauto. intros.
+        exploit alloc_external_symbols_valid_aux.
+        eapply A2. eauto. auto.
+      * clear A1 P1 P2 NOREP.
+        induction gl2.
+        simpl in A2. inv A2.
+        simpl in A2. apply IHgl2. auto.
+    + intros.
+      destruct (symbentry_type e);try congruence.
+      destruct Mem.alloc_glob eqn:ALLOC in A2.
+      destruct store_zeros eqn:STORE in A2.
+      * destruct Mem.drop_perm eqn:DROP in A2.
+        -- exploit alloc_external_symbols_valid_aux.
+           apply A2. eapply Mem.drop_perm_valid_block_1;eauto.
+           unfold Mem.valid_block.
+           erewrite  Genv.store_zeros_support;eauto.
+           apply Mem.support_alloc_glob in ALLOC.
+           rewrite ALLOC.
+           erewrite Mem.sup_incr_glob_in. left.
+           eauto. auto.
+        -- clear A1 P1 P2 NOREP.
+           induction gl2.
+           simpl in A2. inv A2.
+           simpl in A2. apply IHgl2. auto.
+      * clear A1 P1 P2 NOREP.
+        induction gl2.
+        simpl in A2. inv A2.
+        simpl in A2. apply IHgl2. auto.
+    + intros.
+      destruct (symbentry_type e);try congruence.
+      * destruct Mem.alloc_glob eqn:ALLOC in A2.
+        destruct Mem.drop_perm eqn:DROP in A2.
+        -- exploit alloc_external_symbols_valid_aux.
+           apply A2. eapply Mem.drop_perm_valid_block_1;eauto.
+           unfold Mem.valid_block.
+           apply Mem.support_alloc_glob in ALLOC.
+           rewrite ALLOC.
+           erewrite Mem.sup_incr_glob_in. left.
+           eauto. auto.
+        -- clear A1 P1 P2 NOREP.
+           induction gl2.
+           simpl in A2. inv A2.
+           simpl in A2. apply IHgl2. auto.
+      * destruct Mem.alloc_glob eqn:ALLOC in A2.
+        destruct store_zeros eqn:STORE in A2.
+        -- destruct Mem.drop_perm eqn:DROP in A2.
+           ++ exploit alloc_external_symbols_valid_aux.
+              apply A2. eapply Mem.drop_perm_valid_block_1;eauto.
+              unfold Mem.valid_block.
+              erewrite  Genv.store_zeros_support;eauto.
+              apply Mem.support_alloc_glob in ALLOC.
+              rewrite ALLOC.
+              erewrite Mem.sup_incr_glob_in. left.
+              eauto. auto.
+           ++ clear A1 P1 P2 NOREP.
+              induction gl2.
+              simpl in A2. inv A2.
+              simpl in A2. apply IHgl2. auto.
+        --
+          clear A1 P1 P2 NOREP.
+          induction gl2.
+          simpl in A2. inv A2.
+          simpl in A2. apply IHgl2. auto.
+  - clear A1 P1 P2 NOREP.
+    induction gl2.
+    simpl in A2. inv A2.
+    simpl in A2. apply IHgl2. auto.
+Qed.
+
+Lemma find_symbol_not_fresh: forall p id b m ofs,
+    well_formed_symbtbl p.(prog_sectable) p.(prog_symbtable) ->
+    init_mem p = Some m ->
+    Genv.find_symbol (globalenv p) id = Some (b,ofs) ->
+    Mem.valid_block m b.
+Proof.
+  unfold init_mem, globalenv, Genv.find_symbol, gen_symb_map.
+  simpl. intros p id b m ofs MATCH INIT GENV.
+  destr_in INIT.
+  rewrite PTree.gmap in GENV. unfold option_map in GENV.
+  destr_in GENV. inv GENV.
+  unfold gen_global in H0.
+
+  unfold well_formed_symbtbl in MATCH.
+  generalize (MATCH _ _ Heqo0). intros A.  
+  unfold Mem.valid_block.
+  destr_in A.
+  - destruct A as (P1 & sec & P2 & P3 & P4 & P5) .
+    eapply alloc_sections_valid in Heqo;eauto.
+    eapply alloc_external_symbols_valid in INIT;eauto.
+    rewrite Heqs0 in INIT. inv H0. eauto.
+  - eapply alloc_external_symbols_valid in INIT;eauto.
+    destruct A.
+    rewrite Heqs0,H in INIT.
+    inv H0. auto.
+  - destruct A.
+    eapply alloc_external_symbols_valid in INIT;eauto.
+    rewrite Heqs0 in INIT.
+    inv H0. auto.
+Qed.
+
+End INSTRSIZE.
