riscV/RelocProgSemanticsArchi.v
@@ -4,7 +4,7 @@ Require Import Asm RelocProg RelocProgram Globalenvs.
 Require Import Locations Stacklayout Conventions.
 Require Import Linking Errors.
 Require Import LocalLib.
-Require Import RelocProgGlobalenvs RelocProgSemantics.
+Require Import RelocProgGlobalenvs.
 
 Parameter low_half: Genv.t -> ident -> ptrofs -> ptrofs.
 Parameter high_half: Genv.t -> ident -> ptrofs -> val.
@@ -496,18 +496,18 @@ Inductive step (ge: Genv.t): state -> trace -> state -> Prop :=
       Genv.find_instr ge (Vptr b ofs) = Some i ->
       exec_instr ge i rs m = Next rs' m' ->
       step ge (State rs m) E0 (State rs' m')
-  | exec_step_builtin:
-      forall b ofs ef args res rs m vargs t vres rs' m',
-      rs PC = Vptr b ofs ->
-      Genv.find_ext_funct ge (Vptr b ofs) = None ->
-      Genv.find_instr ge (Vptr b ofs) = Some (Pbuiltin ef args res)  ->      
-      eval_builtin_args preg ge rs (rs SP) m args vargs ->
-      external_call ef ge vargs m t vres m' ->
-      rs' = nextinstr (Ptrofs.repr (instr_size (Pbuiltin ef args res)))
-              (set_res res vres
-                (undef_regs (map preg_of (destroyed_by_builtin ef))
-                   (rs#X31 <- Vundef))) ->
-      step ge (State rs m) t (State rs' m')
+  (* | exec_step_builtin: *)
+  (*     forall b ofs ef args res rs m vargs t vres rs' m', *)
+  (*     rs PC = Vptr b ofs -> *)
+  (*     Genv.find_ext_funct ge (Vptr b ofs) = None -> *)
+  (*     Genv.find_instr ge (Vptr b ofs) = Some (Pbuiltin ef args res)  ->       *)
+  (*     eval_builtin_args preg ge rs (rs SP) m args vargs -> *)
+  (*     external_call ef ge vargs m t vres m' -> *)
+  (*     rs' = nextinstr (Ptrofs.repr (instr_size (Pbuiltin ef args res))) *)
+  (*             (set_res res vres *)
+  (*               (undef_regs (map preg_of (destroyed_by_builtin ef)) *)
+  (*                  (rs#X31 <- Vundef))) -> *)
+  (*     step ge (State rs m) t (State rs' m') *)
   | exec_step_external:
       forall b ef args res rs m t rs' m' ofs,
       rs PC = Vptr b ofs ->
@@ -517,89 +517,71 @@ Inductive step (ge: Genv.t): state -> trace -> state -> Prop :=
       rs' = (set_pair (loc_external_result (ef_sig ef) ) res (undef_caller_save_regs rs))#PC <- (rs RA) ->
       step ge (State rs m) t (State rs' m').
 
-Inductive initial_state (p: program): state -> Prop :=
-  | initial_state_intro: forall m0,
-      let ge := globalenv instr_size p in
-      let rs0 :=
-        (Pregmap.init Vundef)
-        # PC <- (Genv.symbol_address ge p.(prog_main) Ptrofs.zero)
-        # SP <- Vnullptr
-        # RA <- Vnullptr in
-      init_mem instr_size p = Some m0 ->
-      initial_state p (State rs0 m0).
-
-Inductive final_state: state -> int -> Prop :=
-  | final_state_intro: forall rs m r,
-      rs PC = Vnullptr ->
-      rs X10 = Vint r ->
-      final_state (State rs m) r.
-
-(* Local Existing Instance mem_accessors_default. *)
-
-Definition semantics p :=
-  Semantics_gen step (initial_state p) final_state (globalenv instr_size p) (Genv.genv_senv (globalenv instr_size p)).
+Inductive initial_state_gen {D: Type} (p: RelocProg.program fundef unit instruction D) (rs: regset) m: state -> Prop :=
+| initial_state_gen_intro:
+  let ge := globalenv instr_size p in
+  let rs0 :=
+    (Pregmap.init Vundef)
+      # PC <- (Genv.symbol_address ge p.(prog_main) Ptrofs.zero)
+      # SP <- Vnullptr
+      # RA <- Vnullptr in
+  initial_state_gen p rs m (State rs0 m).
 
 
-(** Determinacy of the [Asm] semantics. *)
+(** Determinacy of the [Asm] semantics: architecture dependent part . *)
 
-Lemma semantics_determinate: forall p, determinate (semantics p).
-Proof.
 Ltac Equalities :=
   match goal with
   | [ H1: ?a = ?b, H2: ?a = ?c |- _ ] =>
       rewrite H1 in H2; inv H2; Equalities
   | _ => idtac
   end.
-  intros; constructor; simpl; intros.
+  
+Lemma semantics_determinate_step : forall (p:program)  s s1 s2 t1 t2,
+  step (globalenv instr_size p) s t1 s1 ->
+  step (globalenv instr_size p) s t2 s2 -> match_traces (prog_senv p) t1 t2 /\ (t1 = t2 -> s1 = s2).
+Proof.
+   intros.
 - (* determ *)
   inv H; inv H0; Equalities.
-+ split. constructor. auto.
-+ discriminate.
-+ discriminate.
-+ assert (vargs0 = vargs) by (eapply eval_builtin_args_determ; eauto). subst vargs0.
-  exploit external_call_determ. eexact H5. eexact H11. intros [A B].
-  split. auto. intros. destruct B; auto. subst. auto.
-+ assert (args0 = args) by (eapply Asm.extcall_arguments_determ; eauto). subst args0.
+  split. constructor.  auto.
+  assert (args0 = args) by (eapply extcall_arguments_determ; eauto). subst args0.
   exploit external_call_determ. eexact H3. eexact H8. intros [A B].
   split. auto. intros. destruct B; auto. subst. auto.
-- (* trace length *)
-  red; intros; inv H; simpl.
-  lia.
-  eapply external_call_trace_length; eauto.
-  eapply external_call_trace_length; eauto.
-- (* initial states *)
-  inv H; inv H0. assert (m0 = m1) by congruence. subst.
-  f_equal.
-- (* final no step *)
-  assert (NOTNULL: forall b ofs, Vnullptr <> Vptr b ofs).
-  { intros; unfold Vnullptr; destruct Archi.ptr64; congruence. }
-  inv H. red; intros; red; intros. inv H; rewrite H0 in *; eelim NOTNULL; eauto.
-- (* final states *)
-  inv H; inv H0. congruence.
 Qed.
 
-Theorem reloc_prog_single_events p:
-  single_events (semantics p).
+
+Lemma  initial_state_gen_determinate : forall (p: program) rs m s1 s2,
+    initial_state_gen p rs m s1 ->
+    initial_state_gen p rs m s2 ->
+    s1 = s2.
 Proof.
-  red. simpl. intros s t s' STEP.
-  inv STEP; simpl. lia.
-  eapply external_call_trace_length; eauto.
-  eapply external_call_trace_length; eauto.
+  intros. inv H;inv H0.
+  auto.
 Qed.
 
-Theorem reloc_prog_receptive p:
-  receptive (semantics p).
-Proof.
-  split.
-  - simpl. intros s t1 s1 t2 STEP MT.
-    inv STEP.
-    inv MT. eexists. eapply exec_step_internal; eauto.
-    edestruct external_call_receptive as (vres2 & m2 & EC2); eauto.
-    eexists. eapply exec_step_builtin; eauto.
-    edestruct external_call_receptive as (vres2 & m2 & EC2); eauto.
-    eexists. eapply exec_step_external; eauto.
-  - eapply reloc_prog_single_events; eauto.
-Qed.
+(* Theorem reloc_prog_single_events p: *)
+(*   single_events (semantics p). *)
+(* Proof. *)
+(*   red. simpl. intros s t s' STEP. *)
+(*   inv STEP; simpl. lia. *)
+(*   eapply external_call_trace_length; eauto. *)
+(*   eapply external_call_trace_length; eauto. *)
+(* Qed. *)
+
+(* Theorem reloc_prog_receptive p: *)
+(*   receptive (semantics p). *)
+(* Proof. *)
+(*   split. *)
+(*   - simpl. intros s t1 s1 t2 STEP MT. *)
+(*     inv STEP. *)
+(*     inv MT. eexists. eapply exec_step_internal; eauto. *)
+(*     edestruct external_call_receptive as (vres2 & m2 & EC2); eauto. *)
+(*     eexists. eapply exec_step_builtin; eauto. *)
+(*     edestruct external_call_receptive as (vres2 & m2 & EC2); eauto. *)
+(*     eexists. eapply exec_step_external; eauto. *)
+(*   - eapply reloc_prog_single_events; eauto. *)
+(* Qed. *)
 
 
 End WITH_INSTR_SIZE.
