x86/RelocProgSemanticsArchi.v
@@ -4,7 +4,7 @@ Require Import Asm RelocProg RelocProgram Globalenvs.
 Require Import Locations Stacklayout Conventions.
 Require Import Linking Errors.
 Require Import LocalLib.
-Require Import RelocProgGlobalenvs RelocProgSemantics0.
+Require Import RelocProgGlobalenvs .
 
 (** Evaluating an addressing mode *)
 
@@ -571,17 +571,17 @@ Inductive step (ge: Genv.t) : state -> trace -> state -> Prop :=
       Genv.find_instr ge (Vptr b ofs) = Some i ->
       exec_instr ge i rs m = Next rs' m' ->
       step ge (State rs m) E0 (State rs' m')
-| exec_step_builtin:
-    forall b ofs ef args res rs m vargs t vres rs' m',
-      rs PC = Vptr b ofs ->
-      Genv.find_ext_funct ge (Vptr b ofs) = None ->
-      Genv.find_instr ge (Vptr b ofs) = Some (Pbuiltin ef args res)  ->
-      eval_builtin_args preg ge rs (rs RSP) m args vargs ->
-      external_call ef (Genv.genv_senv ge) vargs m t vres m' ->
-      rs' = nextinstr_nf (Ptrofs.repr (instr_size (Pbuiltin ef args res)))
-                         (set_res res vres
-                                  (undef_regs (map preg_of (destroyed_by_builtin ef)) rs)) ->
-        step ge (State rs m) t (State rs' m')
+(* | exec_step_builtin: *)
+(*     forall b ofs ef args res rs m vargs t vres rs' m', *)
+(*       rs PC = Vptr b ofs -> *)
+(*       Genv.find_ext_funct ge (Vptr b ofs) = None -> *)
+(*       Genv.find_instr ge (Vptr b ofs) = Some (Pbuiltin ef args res)  -> *)
+(*       eval_builtin_args preg ge rs (rs RSP) m args vargs -> *)
+(*       external_call ef (Genv.genv_senv ge) vargs m t vres m' -> *)
+(*       rs' = nextinstr_nf (Ptrofs.repr (instr_size (Pbuiltin ef args res))) *)
+(*                          (set_res res vres *)
+(*                                   (undef_regs (map preg_of (destroyed_by_builtin ef)) rs)) -> *)
+(*         step ge (State rs m) t (State rs' m') *)
 | exec_step_external:
     forall b ofs ef args res rs m t rs' m',
       rs PC = Vptr b ofs ->
@@ -603,90 +603,43 @@ Inductive initial_state_gen {D: Type} (p: RelocProg.program fundef unit instruct
     forall m1 m2 stk
       (MALLOC: Mem.alloc m 0 (max_stacksize + align (size_chunk Mptr) 8) = (m1,stk))
       (MST: Mem.storev Mptr m1 (Vptr stk (Ptrofs.repr (max_stacksize + align (size_chunk Mptr) 8 - size_chunk Mptr))) Vnullptr = Some m2),
-      let ge := (globalenv p) in
+      let ge := (globalenv instr_size p) in
       let rs0 :=
           rs # PC <- (Genv.symbol_address ge p.(prog_main) Ptrofs.zero)
            # RA <- Vnullptr
            # RSP <- (Vptr stk (Ptrofs.sub (Ptrofs.repr (max_stacksize + align (size_chunk Mptr) 8)) (Ptrofs.repr (size_chunk Mptr)))) in
       initial_state_gen p rs m (State rs0 m2).
 
-Inductive initial_state (prog: program) (rs: regset) (s: state): Prop :=
-| initial_state_intro: forall m,
-    init_mem prog = Some m ->
-    initial_state_gen prog rs m s ->
-    initial_state prog rs s.
-
-Inductive final_state: state -> int -> Prop :=
-  | final_state_intro: forall rs m r,
-      rs#PC = Vnullptr ->
-      rs#RAX = Vint r ->
-      final_state (State rs m) r.
-
-Definition semantics (p: program) (rs: regset) :=
-  Semantics_gen (step instr_size) (initial_state p rs) final_state (globalenv p) (Genv.genv_senv (globalenv p)).
-
-(** Determinacy of the [Asm] semantics. *)
-
-Lemma semantics_determinate: forall p rs, determinate (semantics p rs).
-Proof.
 Ltac Equalities :=
   match goal with
   | [ H1: ?a = ?b, H2: ?a = ?c |- _ ] =>
       rewrite H1 in H2; inv H2; Equalities
   | _ => idtac
   end.
-  intros; constructor; simpl; intros.
-- (* determ *)
+  
+Lemma semantics_determinate_step : forall (p:program)  s s1 s2 t1 t2,
+  step (globalenv instr_size p) s t1 s1 ->
+  step (globalenv instr_size p) s t2 s2 -> match_traces (prog_senv p) t1 t2 /\ (t1 = t2 -> s1 = s2).
+Proof.
+  intros.
   inv H; inv H0; Equalities.
-+ split. constructor. auto.
-+ discriminate.
-+ discriminate.
-+ assert (vargs0 = vargs) by (eapply eval_builtin_args_determ; eauto). subst vargs0.
-  exploit external_call_determ. eexact H5. eexact H11. intros [A B].
-  split. auto. intros. destruct B; auto. subst. auto.
-+ assert (args0 = args) by (eapply Asm.extcall_arguments_determ; eauto). subst args0.
+  split. constructor.  auto.
+  assert (args0 = args) by (eapply extcall_arguments_determ; eauto). subst args0.
   exploit external_call_determ. eexact H3. eexact H7. intros [A B].
   split. auto. intros. destruct B; auto. subst. auto.
-- (* trace length *)
-  red; intros; inv H; simpl.
-  lia.
-  eapply external_call_trace_length; eauto.
-  eapply external_call_trace_length; eauto.
-- (* initial states *)
-  inv H; inv H0. assert (m = m0) by congruence. subst. inv H2; inv H3.
-  assert (m1 = m3 /\ stk = stk0) by intuition congruence. destruct H0; subst.
-  assert (m2 = m4) by congruence. subst.
-  f_equal. (* congruence. *)
-- (* final no step *)
-  assert (NOTNULL: forall b ofs, Vnullptr <> Vptr b ofs).
-  { intros; unfold Vnullptr; destruct Archi.ptr64; congruence. }
-  inv H. red; intros; red; intros. inv H; rewrite H0 in *; eelim NOTNULL; eauto.
-- (* final states *)
-  inv H; inv H0. congruence.
 Qed.
 
-Theorem reloc_prog_single_events p rs:
-  single_events (semantics p rs).
+Lemma  initial_state_gen_determinate : forall (p: program) rs m s1 s2,
+    initial_state_gen p rs m s1 ->
+    initial_state_gen p rs m s2 ->
+    s1 = s2.
 Proof.
-  red. simpl. intros s t s' STEP.
-  inv STEP; simpl. lia.
-  eapply external_call_trace_length; eauto.
-  eapply external_call_trace_length; eauto.
+  intros. inv H; inv H0. 
+  assert (m1 = m0) by congruence. subst. (* inv H2; inv H3. *)
+  assert (stk = stk0) by intuition congruence. subst.
+  assert (m2 = m3) by congruence. subst.
+  f_equal.
 Qed.
-
-Theorem reloc_prog_receptive p rs:
-  receptive (semantics p rs).
-Proof.
-  split.
-  - simpl. intros s t1 s1 t2 STEP MT.
-    inv STEP.
-    inv MT. eexists. eapply exec_step_internal; eauto.
-    edestruct external_call_receptive as (vres2 & m2 & EC2); eauto.
-    eexists. eapply exec_step_builtin; eauto.
-    edestruct external_call_receptive as (vres2 & m2 & EC2); eauto.
-    eexists. eapply exec_step_external; eauto.
-  - eapply reloc_prog_single_events; eauto.
-Qed.
-
-
+  
+  
 End WITH_INSTR_SIZE.
